3d: separate error code buffer

src/3d/prelude/Actions.fst
@@ -29,24 +29,94 @@ friend Prelude
 open Prelude
 module B = LowStar.Buffer
 
+(* FIXME: Those functions CANNOT be put into a KReMLin root because:
+
+Bundling creates a dependency cycle:
+ResultOps.check_constraint_ok_with_field_id (found in file EverParse) mentions FStar.Monotonic.HyperStack.mem (found in file SHOULDNOTBETHERE)
+FStar.Seq.Base.slice (found in file SHOULDNOTBETHERE) mentions Prims.nat (found in file EverParse)
+Fat
+
+*)
+
+inline_for_extraction
+noextract
+let check_constraint_ok (maybe_fail: B.pointer U64.t) (ok:bool) (position:U32.t) : HST.Stack U32.t
+  (requires (fun h -> B.live h maybe_fail))
+  (ensures (fun h res h' ->
+    B.modifies (if ok then B.loc_none else B.loc_buffer maybe_fail) h h' /\
+    res == position /\
+    ((~ ok) ==> LPL.is_error (B.get h' maybe_fail 0))
+  ))
+=
+      if not ok
+      then B.upd maybe_fail 0ul validator_error_constraint_failed;
+      position
+
+inline_for_extraction
+noextract
+let check_constraint_ok_with_field_id (maybe_fail: B.pointer U64.t) (ok:bool) (startPosition: U32.t) (endPosition:U32.t) (fieldId: field_id) : HST.Stack U32.t
+  (requires (fun h -> B.live h maybe_fail))
+  (ensures (fun h res h' ->
+    B.modifies (if ok then B.loc_none else B.loc_buffer maybe_fail) h h' /\
+    res == (if ok then endPosition else startPosition) /\
+    ((~ ok) ==> LPL.is_error (B.get h' maybe_fail 0))
+  ))
+=
+      if ok
+      then endPosition
+      else begin
+        B.upd maybe_fail 0ul (LPL.set_validator_error_pos_and_code validator_error_constraint_failed 0uL fieldId);
+        startPosition
+      end
+
+inline_for_extraction
+noextract
+let set_error_code
+  (maybe_fail: B.pointer U64.t)
+  (endPosition: U32.t)
+  (startPosition: U32.t)
+  (code: LPL.error_code)
+ : HST.Stack U32.t
+   (requires (fun h -> B.live h maybe_fail))
+   (ensures (fun h res h' ->
+     let is_error = LPL.is_error (B.get h maybe_fail 0) in
+     B.modifies (if is_error then B.loc_buffer maybe_fail else B.loc_none) h h' /\
+     res == (if is_error then startPosition else endPosition) /\
+     (is_error ==> LPL.is_error (B.get h' maybe_fail 0))
+   ))
+  = let maybe_error = B.index maybe_fail 0ul in
+    if LPL.is_error maybe_error
+    then begin
+      if LPL.get_validator_error_code maybe_error = 0uL
+      then B.upd maybe_fail 0ul (LPL.set_validator_error_code maybe_error code);
+      startPosition
+    end else endPosition
+
+
 inline_for_extraction
 let action #nz (#k:parser_kind nz) (#t:Type) (p:parser k t)
            (inv:slice_inv) (l:eloc) (on_success:bool) (a:Type)
-  = #len: U32.t ->
+  =
+    (maybe_fail: B.pointer U64.t) ->
+    #len: U32.t ->
     sl: input_buffer_t len ->
-    pos:LPL.pos_t ->
-    res:U64.t ->
+    pos:U32.t ->
+    res:U32.t ->
     Stack a
       (requires fun h ->
         let open LPL in
+        let is_success = LPL.is_success (B.get h maybe_fail 0) in
+        B.live h maybe_fail /\
+        B.loc_buffer maybe_fail `B.loc_disjoint` LPL.loc_input_buffer sl /\
+        l `B.loc_disjoint` B.loc_buffer maybe_fail /\
         LPL.live_input_buffer h sl /\
         inv (LPL.slice_of sl).LPL.base h /\
         loc_not_unused_in h `loc_includes` l /\
         address_liveness_insensitive_locs `loc_includes` l /\
         l `loc_disjoint` LPL.loc_input_buffer sl /\
-        (U64.v res <= U64.v validator_max_length ==>
-           valid_pos p h (LPL.slice_of sl) (uint64_to_uint32 pos) (uint64_to_uint32 res)) /\
-        (on_success ==> U64.v res <= U64.v validator_max_length))
+        (is_success ==>
+           valid_pos p h (LPL.slice_of sl) pos res) /\
+        (on_success ==> is_success))
       (ensures fun h0 _ h1 ->
         modifies l h0 h1 /\
         h1 `extends` h0 /\
@@ -54,34 +124,38 @@ let action #nz (#k:parser_kind nz) (#t:Type) (p:parser k t)
 
 inline_for_extraction
 let validate_with_action_t #nz (#k:parser_kind nz) (#t:Type) (p:parser k t) (inv:slice_inv) (l:eloc) (allow_reading:bool) =
+  (maybe_fail: B.pointer U64.t) ->
   (#len: U32.t) ->
   (sl: input_buffer_t len) ->
-  (pos: U64.t) ->
-  Stack U64.t
+  (pos: U32.t) ->
+  Stack U32.t
   (requires fun h ->
     let open LPL in
     live_input_buffer h sl /\
     inv (slice_of sl).base h /\
     loc_not_unused_in h `loc_includes` l /\
     address_liveness_insensitive_locs `loc_includes` l /\
-    l `loc_disjoint` LPL.loc_input_buffer sl /\
-    U64.v pos <= U32.v (slice_of sl).len /\
-    R.readable h (perm_of sl) (uint64_to_uint32 pos) (slice_of sl).len
+    l `loc_disjoint` (LPL.loc_input_buffer sl `B.loc_union` B.loc_buffer maybe_fail) /\
+    LPL.loc_input_buffer sl `B.loc_disjoint` B.loc_buffer maybe_fail /\
+    B.live h maybe_fail /\
+    U32.v pos <= U32.v (slice_of sl).len /\
+    R.readable h (perm_of sl) (pos) (slice_of sl).len
   )
   (ensures fun h res h' ->
     let open LPL in
+    let is_success = LPL.is_success (B.get h' maybe_fail 0) in
     h' `extends` h /\
     live_input_buffer h' sl /\
     inv (slice_of sl).base h' /\
-    (is_success res ==> valid_pos p h (slice_of sl) (uint64_to_uint32 pos) (uint64_to_uint32 res)) /\
+    (is_success ==> valid_pos p h (slice_of sl) pos res) /\
     modifies
-      (if allow_reading then l else l `loc_union` (R.loc_perm_from_to (perm_of sl) (uint64_to_uint32 pos) (if is_success res then uint64_to_uint32 res else (slice_of sl).len)))
+      (B.loc_buffer maybe_fail `B.loc_union` (if allow_reading then l else l `loc_union` (R.loc_perm_from_to (perm_of sl) pos (if is_success then res else (slice_of sl).len))))
       h h' /\
-    ((~ allow_reading) ==> R.unreadable h' (perm_of sl) (uint64_to_uint32 pos) (if is_success res then uint64_to_uint32 res else (slice_of sl).len))
+    ((~ allow_reading) ==> R.unreadable h' (perm_of sl) pos (if is_success then res else (slice_of sl).len))
   )
 
 let validate_eta v =
-  fun input startPosition -> v input startPosition
+  fun maybe_fail input startPosition -> v maybe_fail input startPosition
 
 inline_for_extraction noextract
 let act_with_comment
@@ -90,9 +164,9 @@ let act_with_comment
   (#inv:slice_inv) (#l:eloc) (#b:_) (res:Type)
   (a: action p inv l b res)
 : Tot (action p inv l b res)
-= fun input startPosition endPosition ->
+= fun maybe_fail input startPosition endPosition ->
   LPL.comment s;
-  a input startPosition endPosition
+  a maybe_fail input startPosition endPosition
 
 inline_for_extraction
 let leaf_reader
@@ -162,34 +236,48 @@ let validate_drop
    (v: validate_with_action_t p inv l allow_reading)
 : Tot (validate_with_action_t p inv l false)
 = fun
+  maybe_fail
   input
-  (startPosition: U64.t) ->
-  with_drop_if true inv input (LPL.uint64_to_uint32 startPosition) (fun (y: U64.t) -> if LPL.is_success y then LPL.uint64_to_uint32 y else LPL.slice_length input) (v input startPosition)
+  startPosition ->
+  let res = v maybe_fail input startPosition in
+  let to = if LPL.is_success (B.index maybe_fail 0ul) then res else LPL.slice_length input in
+  let h1 = HST.get () in
+  LPL.drop input startPosition to;
+  let h2 = HST.get () in
+  [@inline_let] let _ = assert (h2 `extends` h1) in
+  res
 
+#push-options "--z3rlimit 16"
 inline_for_extraction
 noextract
 let validate_with_success_action' (name: string) #nz (#k1:parser_kind nz) #t1 (#p1:parser k1 t1) (#inv1:_) (#l1:eloc) (#ar:_)
                          (v1:validate_with_action_t p1 inv1 l1 ar)
                          (#inv2:_) (#l2:eloc) #b (a:action p1 inv2 l2 b bool)
   : validate_with_action_t p1 (conj_inv inv1 inv2) (l1 `eloc_union` l2) ar
-  = fun   input
+  = fun   
+        maybe_fail
+        input
         startPosition ->
     let h0 = HST.get () in
     [@(rename_let ("positionAfter" ^ name))]
-    let pos1 = v1 input startPosition in
+    let pos1 = v1 maybe_fail input startPosition in
     let h1 = HST.get () in
     modifies_address_liveness_insensitive_unused_in h0 h1;
-    if LPL.is_success pos1
+    if LPL.is_success (B.index maybe_fail 0ul)
     then
          [@(rename_let ("action_success_" ^ name))]
-         let b = a input startPosition pos1 in
+         let b = a maybe_fail input startPosition pos1 in
          if not b
-         then
-           with_drop_if (not ar) (conj_inv inv1 inv2) input (LPL.uint64_to_uint32 startPosition) (fun _ -> LPL.slice_length input) validator_error_action_failed
-         else
+         then begin
+           B.upd maybe_fail 0ul validator_error_action_failed;
+           let h2 = HST.get () in
+           assert (h2 `extends` h1);
+           with_drop_if (not ar) (conj_inv inv1 inv2) input startPosition (fun _ -> LPL.slice_length input) pos1
+         end else
            pos1
     else
          pos1
+#pop-options
 
 let validate_with_success_action
   name
@@ -197,24 +285,32 @@ let validate_with_success_action
   #inv2 #l2 #b a
 = validate_drop (validate_with_success_action' name v1 a)
 
+#push-options "--z3rlimit 16"
 inline_for_extraction noextract
 let validate_with_error_action' (name: string) #nz (#k1:parser_kind nz) #t1 (#p1:parser k1 t1) (#inv1:_) (#l1:eloc) (#ar:_)
                          (v1:validate_with_action_t p1 inv1 l1 ar)
                          (#inv2:_) (#l2:eloc) (a:action p1 inv2 l2 false bool)
   : validate_with_action_t p1 (conj_inv inv1 inv2) (l1 `eloc_union` l2) ar
-  = fun   input
+  = fun
+        maybe_fail
+        input
         startPosition ->
     let h0 = HST.get () in
     [@(rename_let ("positionAfter" ^ name))]
-    let pos1 = v1 input startPosition in
+    let pos1 = v1 maybe_fail input startPosition in
     let h1 = HST.get () in
     modifies_address_liveness_insensitive_unused_in h0 h1;
-    if LPL.is_success pos1
+    if LPL.is_success (B.index maybe_fail 0ul)
     then pos1
-    else
+    else begin
          [@(rename_let ("action_error_" ^ name))]
-         let b = a input startPosition pos1 in
-         if not b then validator_error_action_failed else pos1
+         let b = a maybe_fail input startPosition pos1 in
+         if not b then B.upd maybe_fail 0ul validator_error_action_failed;
+         let h2 = HST.get () in
+         assert (h2 `extends` h1);
+         pos1
+    end
+#pop-options
 
 let validate_with_error_action
   name
@@ -225,9 +321,9 @@ let validate_with_error_action
 inline_for_extraction noextract
 let validate_ret
   : validate_with_action_t (parse_ret ()) true_inv eloc_none true
-  = fun input startPosition ->
+  = fun maybe_fail input startPosition ->
     let h = HST.get () in
-    [@inline_let] let _ = LPL.valid_facts (parse_ret ()) h (LPL.slice_of input) (LPL.uint64_to_uint32 startPosition) in
+    [@inline_let] let _ = LPL.valid_facts (parse_ret ()) h (LPL.slice_of input) (startPosition) in
     startPosition
 
 #push-options "--z3rlimit 16"
@@ -240,22 +336,26 @@ let validate_pair'
        #nz2 (#k2:parser_kind nz2) #t2 (#p2:parser k2 t2)
        (#inv2:_) (#l2:eloc) (#ar2:_) (v2:validate_with_action_t p2 inv2 l2 ar2)
   : validate_with_action_t (p1 `parse_pair` p2) (conj_inv inv1 inv2) (l1 `eloc_union` l2) (ar1 && ar2)
-  = fun   input
+  = fun   
+        maybe_fail
+        input
         startPosition ->
     let h = HST.get () in
-    [@inline_let] let _ = LPLC.valid_nondep_then h p1 p2 (LPL.slice_of input) (LPL.uint64_to_uint32 startPosition) in
+    [@inline_let] let _ = LPLC.valid_nondep_then h p1 p2 (LPL.slice_of input) (startPosition) in
     [@(rename_let ("positionAfter" ^ name1))]
-    let pos1 = v1 input startPosition in
+    let pos1 = v1 maybe_fail input startPosition in
     let h1 = HST.get () in
     modifies_address_liveness_insensitive_unused_in h h1;
-    if LPL.is_error pos1
+    if LPL.is_error (B.index maybe_fail 0ul)
     then begin
-      with_drop_if (not (ar1 && ar2)) (conj_inv inv1 inv2) input (LPL.uint64_to_uint32 startPosition) (fun _ -> LPL.slice_length input) pos1
+      with_drop_if (not (ar1 && ar2)) (conj_inv inv1 inv2) input (startPosition) (fun _ -> LPL.slice_length input) pos1
     end
     else
-      [@inline_let] let _ = R.readable_split h (LPL.perm_of input) (LPL.uint64_to_uint32 startPosition) (LPL.uint64_to_uint32 pos1) (LPL.slice_length input) in
-      [@inline_let] let _ = LPL.valid_facts p2 h (LPL.slice_of input) (LPL.uint64_to_uint32 pos1) in
-      with_drop_if (not (ar1 && ar2)) (conj_inv inv1 inv2) input (LPL.uint64_to_uint32 startPosition) (fun (x: U64.t) -> if LPL.is_success x then LPL.uint64_to_uint32 x else LPL.slice_length input) (v2 input pos1)
+      [@inline_let] let _ = R.readable_split h (LPL.perm_of input) (startPosition) (pos1) (LPL.slice_length input) in
+      [@inline_let] let _ = LPL.valid_facts p2 h (LPL.slice_of input) (pos1) in
+      let res = v2 maybe_fail input pos1 in
+      let is_success = LPL.is_success (B.index maybe_fail 0ul) in
+      with_drop_if (not (ar1 && ar2)) (conj_inv inv1 inv2) input (startPosition) (fun x -> if is_success then x else LPL.slice_length input) res
 
 let validate_pair
   name1
@@ -271,28 +371,30 @@ let validate_dep_pair
       #nz2 (#k2:parser_kind nz2) (#t2:t1 -> Type) (#p2:(x:t1 -> parser k2 (t2 x)))
       #inv2 #l2 #ar2 (v2:(x:t1 -> validate_with_action_t (p2 x) inv2 l2 ar2))
   : Tot (validate_with_action_t (p1 `parse_dep_pair` p2) (conj_inv inv1 inv2) (l1 `eloc_union` l2) false)
-  = fun input startPosition ->
+  = fun maybe_fail input startPosition ->
       let h = HST.get () in
-      [@inline_let] let _ = LPLC.valid_dtuple2 h p1 p2 (LPL.slice_of input) (LPL.uint64_to_uint32 startPosition) in
+      [@inline_let] let _ = LPLC.valid_dtuple2 h p1 p2 (LPL.slice_of input) (startPosition) in
       [@(rename_let ("positionAfter" ^ name1))]
-      let pos1 = v1 input startPosition in
+      let pos1 = v1 maybe_fail input startPosition in
       let h1 = HST.get() in
-      if LPL.is_error pos1
+      if LPL.is_error (B.index maybe_fail 0ul)
       then begin
-        with_drop_if true (conj_inv inv1 inv2) input (LPL.uint64_to_uint32 startPosition) (fun _ -> LPL.slice_length input) pos1
+        with_drop_if true (conj_inv inv1 inv2) input (startPosition) (fun _ -> LPL.slice_length input) pos1
       end
       else
-        [@inline_let] let _ = R.readable_split h (LPL.perm_of input) (LPL.uint64_to_uint32 startPosition) (LPL.uint64_to_uint32 pos1) (LPL.slice_length input) in
+        [@inline_let] let _ = R.readable_split h (LPL.perm_of input) (startPosition) (pos1) (LPL.slice_length input) in
         [@(rename_let ("" ^ name1))]
-        let x = r1 input (LPL.uint64_to_uint32 startPosition) in
+        let x = r1 input (startPosition) in
         let h15 = HST.get () in
         let _ = modifies_address_liveness_insensitive_unused_in h h15 in
-        [@inline_let] let _ = LPLC.valid_facts (p2 x) h (LPL.slice_of input) (LPL.uint64_to_uint32 pos1) in
-        with_drop_if true (conj_inv inv1 inv2) input (LPL.uint64_to_uint32 startPosition) (fun (y: U64.t) -> if LPL.is_success y then LPL.uint64_to_uint32 y else LPL.slice_length input) (v2 x input pos1)
+        [@inline_let] let _ = LPLC.valid_facts (p2 x) h (LPL.slice_of input) (pos1) in
+        let res = v2 x maybe_fail input pos1 in
+        let is_success = LPL.is_success (B.index maybe_fail 0ul) in
+        with_drop_if true (conj_inv inv1 inv2) input (startPosition) (fun y -> if is_success then y else LPL.slice_length input) res
 
 #pop-options
 
-#push-options "--z3rlimit 32"
+#push-options "--z3rlimit 128"
 
 inline_for_extraction noextract
 let validate_dep_pair_with_refinement_and_action'
@@ -309,28 +411,30 @@ let validate_dep_pair_with_refinement_and_action'
              (conj_inv inv1 (conj_inv inv1' inv2))
              (l1 `eloc_union` (l1' `eloc_union` l2))
              false)
-  = fun input startPosition ->
+  = fun maybe_fail input startPosition ->
       let h0 = HST.get () in
-      [@inline_let] let _ = LPLC.valid_filter h0 p1 f (LPL.slice_of input) (LPL.uint64_to_uint32 startPosition) in
+      [@inline_let] let _ = LPLC.valid_filter h0 p1 f (LPL.slice_of input) (startPosition) in
       [@(rename_let ("positionAfter" ^ name1))]
-      let res = v1 input startPosition in
+      let res = v1 maybe_fail input startPosition in
       let h1 = HST.get() in
       modifies_address_liveness_insensitive_unused_in h0 h1;
-      if LPL.is_error res
+      if LPL.is_error (B.index maybe_fail 0ul)
       then begin
-        with_drop_if true (conj_inv inv1 (conj_inv inv1' inv2)) input (LPL.uint64_to_uint32 startPosition) (fun _ -> LPL.slice_length input) res
+        with_drop_if true (conj_inv inv1 (conj_inv inv1' inv2)) input (startPosition) (fun _ -> LPL.slice_length input) res
       end
       else begin
-        [@inline_let] let _ = R.readable_split h0 (LPL.perm_of input) (LPL.uint64_to_uint32 startPosition) (LPL.uint64_to_uint32 res) (LPL.slice_length input) in
+        [@inline_let] let _ = R.readable_split h0 (LPL.perm_of input) (startPosition) (res) (LPL.slice_length input) in
         [@(rename_let ("" ^ name1))]
-        let field_value = r1 input (LPL.uint64_to_uint32 startPosition) in
+        let field_value = r1 input (startPosition) in
         [@(rename_let (name1 ^ "ConstraintIsOk"))]
         let ok = f field_value in
         [@(rename_let ("pos_or_error_after_" ^ name1))]
-        let res1 = check_constraint_ok_with_field_id ok startPosition res id1 in
-        if LPL.is_error res1
+        let res1 = check_constraint_ok_with_field_id maybe_fail ok startPosition res id1 in
+        let h2 = HST.get () in
+        assert (h2 `extends` h1);
+        if LPL.is_error (B.index maybe_fail 0ul)
         then
-          with_drop_if true (conj_inv inv1 (conj_inv inv1' inv2)) input (LPL.uint64_to_uint32 startPosition) (fun _ -> LPL.slice_length input) res1
+          with_drop_if true (conj_inv inv1 (conj_inv inv1' inv2)) input (startPosition) (fun _ -> LPL.slice_length input) res1
         else let h2 = HST.get() in
              // assert (B.modifies B.loc_none h1 h2);
              // assert (inv1' input.LPL.base h2);
@@ -338,18 +442,28 @@ let validate_dep_pair_with_refinement_and_action'
              // assert (loc_not_unused_in h2 `loc_includes` l1');
              // [@(rename_let ("action_" ^ name1))]
              // let action_result =  in
-             if not (a field_value input startPosition res)
-             then with_drop_if true (conj_inv inv1 (conj_inv inv1' inv2)) input (LPL.uint64_to_uint32 startPosition) (fun _ -> LPL.slice_length input) (LPL.set_validator_error_pos_and_code validator_error_action_failed startPosition id1) //action failed
-             else begin
+             if not (a field_value maybe_fail input startPosition res)
+             then begin
+               B.upd maybe_fail 0ul (LPL.set_validator_error_pos_and_code validator_error_action_failed 0uL id1);
+               let h3 = HST.get () in
+               assert (h3 `extends` h2);
+               with_drop_if true (conj_inv inv1 (conj_inv inv1' inv2)) input (startPosition) (fun _ -> LPL.slice_length input) startPosition //action failed
+             end else begin
                let open LPL in
                // assert (valid_pos (p1 `(LPC.parse_filter #k1 #t1)` f) h0 input (uint64_to_uint32 pos) (uint64_to_uint32 res));
                let h15 = HST.get () in
                let _ = modifies_address_liveness_insensitive_unused_in h0 h15 in
-               [@inline_let] let _ = LPLC.valid_facts (p2 field_value) h0 (LPL.slice_of input) (LPL.uint64_to_uint32 res1) in
-               [@inline_let] let _ = LPLC.valid_dtuple2 h0 (p1 `LPC.parse_filter` f) p2 (LPL.slice_of input) (LPL.uint64_to_uint32 startPosition) in
-               with_drop_if true (conj_inv inv1 (conj_inv inv1' inv2)) input (LPL.uint64_to_uint32 startPosition) (fun (x: U64.t) -> if LPL.is_success x then LPL.uint64_to_uint32 x else LPL.slice_length input) (v2 field_value input res1)
+               [@inline_let] let _ = LPLC.valid_facts (p2 field_value) h0 (LPL.slice_of input) (res1) in
+               [@inline_let] let _ = LPLC.valid_dtuple2 h0 (p1 `LPC.parse_filter` f) p2 (LPL.slice_of input) (startPosition) in
+               let res = v2 field_value maybe_fail input res1 in
+               let is_success = LPL.is_success (B.index maybe_fail 0ul) in
+               with_drop_if true (conj_inv inv1 (conj_inv inv1' inv2)) input (startPosition) (fun x -> if is_success then x else LPL.slice_length input) res
              end
         end
+
+#pop-options
+
+#push-options "--z3rlimit 64"
 
 inline_for_extraction noextract
 let validate_dep_pair_with_refinement_and_action_total_zero_parser'
@@ -372,23 +486,25 @@ let validate_dep_pair_with_refinement_and_action_total_zero_parser'
            k1.parser_kind_metadata == Some ParserKindMetadataTotal
          ))
          (ensures (fun _ -> True))
-  = fun input startPosition ->
+  = fun maybe_fail input startPosition ->
       let h0 = HST.get () in
-      [@inline_let] let _ = LPLC.valid_filter h0 p1 f (LPL.slice_of input) (LPL.uint64_to_uint32 startPosition) in
-      [@inline_let] let _ = LPLC.valid_facts p1 h0 (LPL.slice_of input) (LPL.uint64_to_uint32 startPosition) in
+      [@inline_let] let _ = LPLC.valid_filter h0 p1 f (LPL.slice_of input) (startPosition) in
+      [@inline_let] let _ = LPLC.valid_facts p1 h0 (LPL.slice_of input) (startPosition) in
       [@inline_let] let _ = LP.parser_kind_prop_equiv k1 p1 in
       begin
         LowStar.Comment.comment ("Validating field " ^ name1);
-        [@inline_let] let _ = R.readable_split h0 (LPL.perm_of input) (LPL.uint64_to_uint32 startPosition) (LPL.uint64_to_uint32 startPosition) (LPL.slice_length input) in
+        [@inline_let] let _ = R.readable_split h0 (LPL.perm_of input) (startPosition) (startPosition) (LPL.slice_length input) in
         [@(rename_let ("" ^ name1))]
-        let field_value = r1 input (LPL.uint64_to_uint32 startPosition) in
+        let field_value = r1 input (startPosition) in
         [@(rename_let (name1 ^ "ConstraintIsOk"))]
         let ok = f field_value in
         [@(rename_let ("pos_or_error_after_" ^ name1))]
-        let res1 = check_constraint_ok_with_field_id ok startPosition startPosition id1 in
-        if LPL.is_error res1
+        let res1 = check_constraint_ok_with_field_id maybe_fail ok startPosition startPosition id1 in
+        let h1 = HST.get () in
+        assert (h1 `extends` h0);
+        if LPL.is_error (B.index maybe_fail 0ul)
         then
-             with_drop_if true (conj_inv inv1 (conj_inv inv1' inv2)) input (LPL.uint64_to_uint32 startPosition) (fun _ -> LPL.slice_length input) res1
+             with_drop_if true (conj_inv inv1 (conj_inv inv1' inv2)) input (startPosition) (fun _ -> LPL.slice_length input) res1
         else let h2 = HST.get() in
              // assert (B.modifies B.loc_none h1 h2);
              // assert (inv1' input.LPL.base h2);
@@ -396,16 +512,22 @@ let validate_dep_pair_with_refinement_and_action_total_zero_parser'
              // assert (loc_not_unused_in h2 `loc_includes` l1');
              // [@(rename_let ("action_" ^ name1))]
              // let action_result =  in
-             if not (a field_value input startPosition startPosition)
-             then with_drop_if true (conj_inv inv1 (conj_inv inv1' inv2)) input (LPL.uint64_to_uint32 startPosition) (fun _ -> LPL.slice_length input) (LPL.set_validator_error_pos_and_code validator_error_action_failed startPosition id1) //action failed
-             else begin
+             if not (a field_value maybe_fail input startPosition startPosition)
+             then begin
+               B.upd maybe_fail 0ul (LPL.set_validator_error_pos_and_code validator_error_action_failed 0uL id1);
+               let h3 = HST.get () in
+               assert (h3 `extends` h2);
+               with_drop_if true (conj_inv inv1 (conj_inv inv1' inv2)) input (startPosition) (fun _ -> LPL.slice_length input) startPosition //action failed
+             end else begin
                let open LPL in
                // assert (valid_pos (p1 `(LPC.parse_filter #k1 #t1)` f) h0 input (uint64_to_uint32 pos) (uint64_to_uint32 res));
                let h15 = HST.get () in
                let _ = modifies_address_liveness_insensitive_unused_in h0 h15 in
-               [@inline_let] let _ = LPLC.valid_facts (p2 field_value) h0 (LPL.slice_of input) (LPL.uint64_to_uint32 res1) in
-               [@inline_let] let _ = LPLC.valid_dtuple2 h0 (p1 `LPC.parse_filter` f) p2 (LPL.slice_of input) (LPL.uint64_to_uint32 startPosition) in
-               with_drop_if true (conj_inv inv1 (conj_inv inv1' inv2)) input (LPL.uint64_to_uint32 startPosition) (fun (x: U64.t) -> if LPL.is_success x then LPL.uint64_to_uint32 x else LPL.slice_length input) (v2 field_value input res1)
+               [@inline_let] let _ = LPLC.valid_facts (p2 field_value) h0 (LPL.slice_of input) (res1) in
+               [@inline_let] let _ = LPLC.valid_dtuple2 h0 (p1 `LPC.parse_filter` f) p2 (LPL.slice_of input) (startPosition) in
+               let res = v2 field_value maybe_fail input res1 in
+               let is_success = LPL.is_success (B.index maybe_fail 0ul) in
+               with_drop_if true (conj_inv inv1 (conj_inv inv1' inv2)) input (startPosition) (fun x -> if is_success then x else LPL.slice_length input) res
              end
         end
 
@@ -423,28 +545,30 @@ let validate_dep_pair_with_refinement'
              (conj_inv inv1 inv2)
              (l1 `eloc_union` l2)
              false)
-  = fun input startPosition ->
+  = fun maybe_fail input startPosition ->
       let h0 = HST.get () in
-      [@inline_let] let _ = LPLC.valid_filter h0 p1 f (LPL.slice_of input) (LPL.uint64_to_uint32 startPosition) in
+      [@inline_let] let _ = LPLC.valid_filter h0 p1 f (LPL.slice_of input) (startPosition) in
       [@(rename_let ("positionAfter" ^ name1))]
-      let res = v1 input startPosition in
+      let res = v1 maybe_fail input startPosition in
       let h1 = HST.get() in
       modifies_address_liveness_insensitive_unused_in h0 h1;
-      if LPL.is_error res
+      if LPL.is_error (B.index maybe_fail 0ul)
       then begin
-        with_drop_if true (conj_inv inv1 inv2) input (LPL.uint64_to_uint32 startPosition) (fun _ -> LPL.slice_length input) res
+        with_drop_if true (conj_inv inv1 inv2) input (startPosition) (fun _ -> LPL.slice_length input) res
       end
       else begin
-        [@inline_let] let _ = R.readable_split h0 (LPL.perm_of input) (LPL.uint64_to_uint32 startPosition) (LPL.uint64_to_uint32 res) (LPL.slice_length input) in
+        [@inline_let] let _ = R.readable_split h0 (LPL.perm_of input) (startPosition) (res) (LPL.slice_length input) in
         [@(rename_let ("" ^ name1))]
-        let field_value = r1 input (LPL.uint64_to_uint32 startPosition) in
+        let field_value = r1 input (startPosition) in
         [@(rename_let (name1 ^ "ConstraintIsOk"))]
         let ok = f field_value in
-        [@(rename_let ("positionOrErrorAfter" ^ name1))]
-        let res1 = check_constraint_ok_with_field_id ok startPosition res id1 in
-        if LPL.is_error res1
+        [@(rename_let ("positionAfter" ^ name1))]
+        let res1 = check_constraint_ok_with_field_id maybe_fail ok startPosition res id1 in
+        let h1 = HST.get () in
+        assert (h1 `extends` h0);
+        if LPL.is_error (B.index maybe_fail 0ul)
         then
-             with_drop_if true (conj_inv inv1 inv2) input (LPL.uint64_to_uint32 startPosition) (fun _ -> LPL.slice_length input) res1
+             with_drop_if true (conj_inv inv1 inv2) input (startPosition) (fun _ -> LPL.slice_length input) res1
         else let h2 = HST.get() in
              // assert (B.modifies B.loc_none h1 h2);
              // assert (inv1' input.LPL.base h2);
@@ -454,9 +578,11 @@ let validate_dep_pair_with_refinement'
              // assert (valid_pos (p1 `(LPC.parse_filter #k1 #t1)` f) h0 input (uint64_to_uint32 pos) (uint64_to_uint32 res));
              let h15 = HST.get () in
              let _ = modifies_address_liveness_insensitive_unused_in h0 h15 in
-             [@inline_let] let _ = LPLC.valid_facts (p2 field_value) h0 (LPL.slice_of input) (LPL.uint64_to_uint32 res1) in
-             [@inline_let] let _ = LPLC.valid_dtuple2 h0 (p1 `LPC.parse_filter` f) p2 (LPL.slice_of input) (LPL.uint64_to_uint32 startPosition) in
-             with_drop_if true (conj_inv inv1 inv2) input (LPL.uint64_to_uint32 startPosition) (fun (y: U64.t) -> if LPL.is_success y then LPL.uint64_to_uint32 y else LPL.slice_length input) (v2 field_value input res1)
+             [@inline_let] let _ = LPLC.valid_facts (p2 field_value) h0 (LPL.slice_of input) (res1) in
+             [@inline_let] let _ = LPLC.valid_dtuple2 h0 (p1 `LPC.parse_filter` f) p2 (LPL.slice_of input) (startPosition) in
+             let res = v2 field_value maybe_fail input res1 in
+             let is_success = LPL.is_success (B.index maybe_fail 0ul) in
+             with_drop_if true (conj_inv inv1 inv2) input (startPosition) (fun y -> if is_success then y else LPL.slice_length input) (res)
         end
 
 inline_for_extraction noextract
@@ -479,22 +605,24 @@ let validate_dep_pair_with_refinement_total_zero_parser'
            k1.parser_kind_metadata == Some ParserKindMetadataTotal
          ))
          (ensures (fun _ -> True))
-  = fun input startPosition ->
+  = fun maybe_fail input startPosition ->
       let h0 = HST.get () in
-      [@inline_let] let _ = LPLC.valid_filter h0 p1 f (LPL.slice_of input) (LPL.uint64_to_uint32 startPosition) in
-      [@inline_let] let _ = LPLC.valid_facts p1 h0 (LPL.slice_of input) (LPL.uint64_to_uint32 startPosition) in
+      [@inline_let] let _ = LPLC.valid_filter h0 p1 f (LPL.slice_of input) (startPosition) in
+      [@inline_let] let _ = LPLC.valid_facts p1 h0 (LPL.slice_of input) (startPosition) in
       [@inline_let] let _ = LP.parser_kind_prop_equiv k1 p1 in
       begin
         LowStar.Comment.comment ("Validating field " ^ name1);
-        [@inline_let] let _ = R.readable_split h0 (LPL.perm_of input) (LPL.uint64_to_uint32 startPosition) (LPL.uint64_to_uint32 startPosition) (LPL.slice_length input) in
+        [@inline_let] let _ = R.readable_split h0 (LPL.perm_of input) (startPosition) (startPosition) (LPL.slice_length input) in
         [@(rename_let ("" ^ name1))]
-        let field_value = r1 input (LPL.uint64_to_uint32 startPosition) in
+        let field_value = r1 input (startPosition) in
         [@(rename_let (name1 ^ "ConstraintIsOk"))]
         let ok = f field_value in
-        [@(rename_let ("positionOrErrorAfter" ^ name1))]
-        let res1 = check_constraint_ok_with_field_id ok startPosition startPosition id1 in
-        if LPL.is_error res1
-        then with_drop_if true (conj_inv inv1 inv2) input (LPL.uint64_to_uint32 startPosition) (fun _ -> LPL.slice_length input) res1
+        [@(rename_let ("positionAfter" ^ name1))]
+        let res1 = check_constraint_ok_with_field_id maybe_fail ok startPosition startPosition id1 in
+        let h1 = HST.get () in
+        assert (h1 `extends` h0);
+        if LPL.is_error (B.index maybe_fail 0ul)
+        then with_drop_if true (conj_inv inv1 inv2) input (startPosition) (fun _ -> LPL.slice_length input) res1
         else let h2 = HST.get() in
              // assert (B.modifies B.loc_none h1 h2);
              // assert (inv1' input.LPL.base h2);
@@ -504,9 +632,11 @@ let validate_dep_pair_with_refinement_total_zero_parser'
              // assert (valid_pos (p1 `(LPC.parse_filter #k1 #t1)` f) h0 input (uint64_to_uint32 pos) (uint64_to_uint32 res));
              let h15 = HST.get () in
              let _ = modifies_address_liveness_insensitive_unused_in h0 h15 in
-             [@inline_let] let _ = LPLC.valid_facts (p2 field_value) h0 (LPL.slice_of input) (LPL.uint64_to_uint32 res1) in
-             [@inline_let] let _ = LPLC.valid_dtuple2 h0 (p1 `LPC.parse_filter` f) p2 (LPL.slice_of input) (LPL.uint64_to_uint32 startPosition) in
-             with_drop_if true (conj_inv inv1 inv2) input (LPL.uint64_to_uint32 startPosition) (fun (y: U64.t) -> if LPL.is_success y then LPL.uint64_to_uint32 y else LPL.slice_length input) (v2 field_value input res1)
+             [@inline_let] let _ = LPLC.valid_facts (p2 field_value) h0 (LPL.slice_of input) (res1) in
+             [@inline_let] let _ = LPLC.valid_dtuple2 h0 (p1 `LPC.parse_filter` f) p2 (LPL.slice_of input) (startPosition) in
+             let res = v2 field_value maybe_fail input res1 in
+             let is_success = LPL.is_success (B.index maybe_fail 0ul) in
+             with_drop_if true (conj_inv inv1 inv2) input (startPosition) (fun y -> if is_success then y else LPL.slice_length input) (res)
         end
 
 #pop-options
@@ -535,7 +665,7 @@ let validate_dep_pair_with_refinement_and_action
     else
       validate_dep_pair_with_refinement_and_action' name1 id1 v1 r1 f a v2
 
-#push-options "--z3rlimit 32"
+#push-options "--z3rlimit 64"
 
 inline_for_extraction noextract
 let validate_dep_pair_with_action
@@ -549,29 +679,35 @@ let validate_dep_pair_with_action
              (conj_inv inv1 (conj_inv inv1' inv2))
              (l1 `eloc_union` (l1' `eloc_union` l2))
              false)
-  = fun input startPosition ->
+  = fun maybe_fail input startPosition ->
       let h0 = HST.get () in
-      let res = v1 input startPosition in
+      let res = v1 maybe_fail input startPosition in
       let h1 = HST.get() in
       modifies_address_liveness_insensitive_unused_in h0 h1;
-      if LPL.is_error res
+      if LPL.is_error (B.index maybe_fail 0ul)
       then begin
-        with_drop_if true (conj_inv inv1 (conj_inv inv1' inv2)) input (LPL.uint64_to_uint32 startPosition) (fun _ -> LPL.slice_length input) res
+        with_drop_if true (conj_inv inv1 (conj_inv inv1' inv2)) input (startPosition) (fun _ -> LPL.slice_length input) res
       end
       else begin
-        [@inline_let] let _ = R.readable_split h0 (LPL.perm_of input) (LPL.uint64_to_uint32 startPosition) (LPL.uint64_to_uint32 res) (LPL.slice_length input) in
-        let field_value = r1 input (LPL.uint64_to_uint32 startPosition) in
+        [@inline_let] let _ = R.readable_split h0 (LPL.perm_of input) (startPosition) (res) (LPL.slice_length input) in
+        let field_value = r1 input (startPosition) in
         let h2 = HST.get() in
         modifies_address_liveness_insensitive_unused_in h1 h2;
-        let action_result = a field_value input startPosition res in
+        let action_result = a field_value maybe_fail input startPosition res in
         if not action_result
-        then with_drop_if true (conj_inv inv1 (conj_inv inv1' inv2)) input (LPL.uint64_to_uint32 startPosition) (fun _ -> LPL.slice_length input) validator_error_action_failed //action failed
-        else begin
+        then begin
+          B.upd maybe_fail 0ul validator_error_action_failed;
+          let h2 = HST.get () in
+          assert (h2 `extends` h1);
+          with_drop_if true (conj_inv inv1 (conj_inv inv1' inv2)) input (startPosition) (fun _ -> LPL.slice_length input) startPosition //action failed
+        end else begin
                let open LPL in
                let h15 = HST.get () in
                let _ = modifies_address_liveness_insensitive_unused_in h0 h15 in
-               [@inline_let] let _ = LPLC.valid_dtuple2 h0 p1 p2 (LPL.slice_of input) (LPL.uint64_to_uint32 startPosition) in
-               with_drop_if true (conj_inv inv1 (conj_inv inv1' inv2)) input (LPL.uint64_to_uint32 startPosition) (fun (y: U64.t) -> if LPL.is_success y then LPL.uint64_to_uint32 y else LPL.slice_length input) (v2 field_value input res)
+               [@inline_let] let _ = LPLC.valid_dtuple2 h0 p1 p2 (LPL.slice_of input) (startPosition) in
+               let res = v2 field_value maybe_fail input res in
+               let is_success = LPL.is_success (B.index maybe_fail 0ul) in
+               with_drop_if true (conj_inv inv1 (conj_inv inv1' inv2)) input (startPosition) (fun y -> if is_success then y else LPL.slice_length input) (res)
              end
       end
 
@@ -605,24 +741,28 @@ let validate_filter' (name: string) #nz (#k:parser_kind nz) (#t:_) (#p:parser k 
                     #inv #l (v:validate_with_action_t p inv l true)
                     (r:leaf_reader p) (f:t -> bool) (cr:string) (cf:string)
   : Tot (validate_with_action_t #nz (p `LPC.parse_filter` f) inv l false)
-  = fun input startPosition ->
+  = fun maybe_fail input startPosition ->
     let h = HST.get () in
-    [@inline_let] let _ = LPLC.valid_filter h p f (LPL.slice_of input) (LPL.uint64_to_uint32 startPosition) in
+    [@inline_let] let _ = LPLC.valid_filter h p f (LPL.slice_of input) (startPosition) in
     [@(rename_let ("positionAfter" ^ name))]
-    let res = v input startPosition in
+    let res = v maybe_fail input startPosition in
     let h1 = HST.get () in
-    if LPL.is_error res
-    then with_drop_if true inv input (LPL.uint64_to_uint32 startPosition) (fun _ -> LPL.slice_length input) res
+    if LPL.is_error (B.index maybe_fail 0ul)
+    then with_drop_if true inv input (startPosition) (fun _ -> LPL.slice_length input) res
     else begin
       LowStar.Comment.comment cr;
-      [@inline_let] let _ = R.readable_split h (LPL.perm_of input) (LPL.uint64_to_uint32 startPosition) (LPL.uint64_to_uint32 res) (LPL.slice_length input) in
+      [@inline_let] let _ = R.readable_split h (LPL.perm_of input) (startPosition) (res) (LPL.slice_length input) in
       [@(rename_let ("" ^ name))]
-      let field_value = r input (LPL.uint64_to_uint32 startPosition) in
+      let field_value = r input (startPosition) in
       LowStar.Comment.comment (normalize_term ("start: " ^cf));
       [@(rename_let (name ^ "ConstraintIsOk"))]
       let ok = f field_value in
       LowStar.Comment.comment (normalize_term ("end: " ^ cf));
-      with_drop_if true inv input (LPL.uint64_to_uint32 startPosition) (fun (y: U64.t) -> if LPL.is_success y then LPL.uint64_to_uint32 y else LPL.slice_length input) (check_constraint_ok ok res)
+      let res = check_constraint_ok maybe_fail ok res in
+      let is_success = LPL.is_success (B.index maybe_fail 0ul) in
+      let h2 = HST.get () in
+      assert (h2 `extends` h1);
+      with_drop_if true inv input (startPosition) (fun y -> if is_success then y else LPL.slice_length input) (res)
     end
 
 inline_for_extraction noextract
@@ -632,6 +772,7 @@ let validate_filter (name: string) #nz (#k:parser_kind nz) (#t:_) (#p:parser k t
   : Tot (validate_with_action_t (p `parse_filter` f) inv l false)
   = validate_filter' name v r f cr cf
 
+#push-options "--z3rlimit 16"
 inline_for_extraction noextract
 let validate_filter'_with_action
                     (name: string) #nz (#k:parser_kind nz) (#t:_) (#p:parser k t)
@@ -639,19 +780,19 @@ let validate_filter'_with_action
                     (r:leaf_reader p) (f:t -> bool) (cr:string) (cf:string)
                     (#b:bool) #inva (#la:eloc) (a: t -> action #nz #(filter_kind k) #_ (p `LPC.parse_filter` f) inva la b bool)
   : Tot (validate_with_action_t #nz (p `LPC.parse_filter` f) (conj_inv inv inva) (eloc_union l la) false)
-  = fun input startPosition ->
+  = fun maybe_fail input startPosition ->
     let h = HST.get () in
-    [@inline_let] let _ = LPLC.valid_filter h p f (LPL.slice_of input) (LPL.uint64_to_uint32 startPosition) in
+    [@inline_let] let _ = LPLC.valid_filter h p f (LPL.slice_of input) (startPosition) in
     [@(rename_let ("positionAfter" ^ name))]
-    let res = v input startPosition in
+    let res = v maybe_fail input startPosition in
     let h1 = HST.get () in
-    if LPL.is_error res
-    then with_drop_if true (conj_inv inv inva) input (LPL.uint64_to_uint32 startPosition) (fun _ -> LPL.slice_length input) res
+    if LPL.is_error (B.index maybe_fail 0ul)
+    then with_drop_if true (conj_inv inv inva) input (startPosition) (fun _ -> LPL.slice_length input) res
     else begin
       LowStar.Comment.comment cr;
-      [@inline_let] let _ = R.readable_split h (LPL.perm_of input) (LPL.uint64_to_uint32 startPosition) (LPL.uint64_to_uint32 res) (LPL.slice_length input) in
+      [@inline_let] let _ = R.readable_split h (LPL.perm_of input) (startPosition) (res) (LPL.slice_length input) in
       [@(rename_let ("" ^ name))]
-      let field_value = r input (LPL.uint64_to_uint32 startPosition) in
+      let field_value = r input (startPosition) in
       LowStar.Comment.comment (normalize_term ("start: " ^cf));
       [@(rename_let (name ^ "ConstraintIsOk"))]
       let ok = f field_value in
@@ -659,11 +800,22 @@ let validate_filter'_with_action
       if ok
         then let h15 = HST.get () in
              let _ = modifies_address_liveness_insensitive_unused_in h h15 in
-             if a field_value input startPosition res
+             if a field_value maybe_fail input startPosition res
              then res
-             else with_drop_if true (conj_inv inv inva) input (LPL.uint64_to_uint32 startPosition) (fun _ -> LPL.slice_length input) validator_error_action_failed
-      else with_drop_if true (conj_inv inv inva) input (LPL.uint64_to_uint32 startPosition) (fun _ -> LPL.slice_length input) validator_error_constraint_failed
+             else begin
+               B.upd maybe_fail 0ul validator_error_action_failed;
+               let h2 = HST.get () in
+               assert (h2 `extends` h1);
+               with_drop_if true (conj_inv inv inva) input (startPosition) (fun _ -> LPL.slice_length input) res
+             end
+      else begin
+        B.upd maybe_fail 0ul validator_error_constraint_failed;
+        let h2 = HST.get () in
+        assert (h2 `extends` h1);
+        with_drop_if true (conj_inv inv inva) input (startPosition) (fun _ -> LPL.slice_length input) res
+      end
     end
+#pop-options
 
 inline_for_extraction noextract
 let validate_filter_with_action
@@ -674,7 +826,7 @@ let validate_filter_with_action
   : Tot (validate_with_action_t #nz (p `parse_filter` f) (conj_inv inv inva) (eloc_union l la) false)
   = validate_filter'_with_action name v r f cr cf a
 
-
+#push-options "--z3rlimit 16"
 inline_for_extraction noextract
 let validate_with_dep_action
                     (name: string) #nz (#k:parser_kind nz) (#t:_) (#p:parser k t)
@@ -682,35 +834,41 @@ let validate_with_dep_action
                     (r:leaf_reader p)
                     (#b:bool) #inva (#la:eloc) (a: t -> action p inva la b bool)
   : Tot (validate_with_action_t #nz p (conj_inv inv inva) (eloc_union l la) false)
-  = fun input startPosition ->
+  = fun maybe_fail input startPosition ->
     let h = HST.get () in
     [@(rename_let ("positionAfter" ^ name))]
-    let res = v input startPosition in
+    let res = v maybe_fail input startPosition in
     let h1 = HST.get () in
-    if LPL.is_error res
-    then with_drop_if true (conj_inv inv inva) input (LPL.uint64_to_uint32 startPosition) (fun _ -> LPL.slice_length input) res
+    if LPL.is_error (B.index maybe_fail 0ul)
+    then with_drop_if true (conj_inv inv inva) input (startPosition) (fun _ -> LPL.slice_length input) res
     else begin
-      [@inline_let] let _ = R.readable_split h (LPL.perm_of input) (LPL.uint64_to_uint32 startPosition) (LPL.uint64_to_uint32 res) (LPL.slice_length input) in
+      [@inline_let] let _ = R.readable_split h (LPL.perm_of input) (startPosition) (res) (LPL.slice_length input) in
       [@(rename_let ("" ^ name))]
-      let field_value = r input (LPL.uint64_to_uint32 startPosition) in
+      let field_value = r input (startPosition) in
       let h15 = HST.get () in
       let _ = modifies_address_liveness_insensitive_unused_in h h15 in
-      if a field_value input startPosition res
+      if a field_value maybe_fail input startPosition res
       then res
-      else with_drop_if true (conj_inv inv inva) input (LPL.uint64_to_uint32 startPosition) (fun _ -> LPL.slice_length input) validator_error_action_failed
+      else begin
+        B.upd maybe_fail 0ul validator_error_action_failed;
+        let h2 = HST.get () in
+        assert (h2 `extends` h1);
+        with_drop_if true (conj_inv inv inva) input (startPosition) (fun _ -> LPL.slice_length input) res
+      end
     end
+#pop-options
 
 inline_for_extraction noextract
 let validate_weaken #nz (#k:parser_kind nz) #t (#p:parser k t)
                     #inv #l #ar (v:validate_with_action_t p inv l ar)
                     #nz' (k':parser_kind nz'{k' `is_weaker_than` k})
   : Tot (validate_with_action_t (parse_weaken p k') inv l ar)
-  = fun input startPosition ->
+  = fun maybe_fail input startPosition ->
     let open LPLC in
     let h = HST.get () in
     [@inline_let]
-    let _ = valid_weaken k' p h (LPL.slice_of input) (LPL.uint64_to_uint32 startPosition) in
-    v input startPosition
+    let _ = valid_weaken k' p h (LPL.slice_of input) (startPosition) in
+    v maybe_fail input startPosition
 
 /// Parser: weakening kinds
 inline_for_extraction noextract
@@ -743,15 +901,21 @@ let validate_weaken_right (#nz:_) (#k:parser_kind nz) (#t:_) (#p:parser k t)
 inline_for_extraction noextract
 let validate_impos ()
   : Tot (validate_with_action_t (parse_impos ()) true_inv eloc_none true)
-  = fun _ _ -> validator_error_impossible
+  = fun maybe_fail _ startPosition -> 
+    B.upd maybe_fail 0ul validator_error_impossible;
+    startPosition
 
 inline_for_extraction noextract
 let validate_with_error #nz (#k:parser_kind nz) #t (#p:parser k t)
                         #inv #l #ar (c:field_id) (v:validate_with_action_t p inv l ar)
   : Tot (validate_with_action_t p inv l ar)
-  = fun input startPosition ->
-    let endPositionOrError = v input startPosition in
-    LPL.maybe_set_error_code endPositionOrError startPosition c
+  = fun maybe_fail input startPosition ->
+    let h0 = HST.get () in
+    let endPosition = v maybe_fail input startPosition in
+    let res = set_error_code maybe_fail endPosition startPosition c in
+    let h1 = HST.get () in
+    assert (h1 `extends` h0);
+    res
 
 noextract inline_for_extraction
 let validate_ite #nz (#k:parser_kind nz) (#a:Type) (#b:Type)
@@ -760,8 +924,8 @@ let validate_ite #nz (#k:parser_kind nz) (#a:Type) (#b:Type)
                  (p1:squash e -> parser k a) (v1:(squash e -> validate_with_action_t (p1()) inv1 l1 ar1))
                  (p2:squash (not e) -> parser k b) (v2:(squash (not e) -> validate_with_action_t (p2()) inv2 l2 ar2))
   : Tot (validate_with_action_t (parse_ite e p1 p2) (conj_inv inv1 inv2) (l1 `eloc_union` l2) false)
-  = fun input startPosition ->
-      if e then validate_drop (v1 ()) input startPosition else validate_drop (v2 ()) input startPosition
+  = fun maybe_fail input startPosition ->
+      if e then validate_drop (v1 ()) maybe_fail input startPosition else validate_drop (v2 ()) maybe_fail input startPosition
 
 unfold
 let validate_list_inv
@@ -771,42 +935,48 @@ let validate_list_inv
   (inv: slice_inv)
   (l: loc)
   (g0 g1: Ghost.erased HS.mem)
+  (maybe_fail: pointer U64.t)
   (#len: U32.t)
   (sl: input_buffer_t len)
   (pos0: U32.t)
-  (bpos: pointer U64.t)
+  (bpos: pointer U32.t)
   (h: HS.mem)
   (stop: bool)
 : GTot Type0
 = let h0 = Ghost.reveal g0 in
   let h1 = Ghost.reveal g1 in
   let pos1 = Seq.index (as_seq h bpos) 0 in
+  let err = B.get h maybe_fail 0 in
   inv (LPL.slice_of sl).LPL.base h0 /\
   h `extends` h0 /\
   loc_not_unused_in h0 `loc_includes` l /\
   l `loc_disjoint` LPL.loc_input_buffer sl /\
   l `loc_disjoint` loc_buffer bpos /\
+  l `loc_disjoint` loc_buffer maybe_fail /\
   address_liveness_insensitive_locs `loc_includes` l /\
   B.loc_buffer bpos `B.loc_disjoint` LPL.loc_input_buffer sl /\
+  B.loc_buffer bpos `B.loc_disjoint` B.loc_buffer maybe_fail /\
+  LPL.loc_input_buffer sl `B.loc_disjoint` B.loc_buffer maybe_fail /\
   k.LPL.parser_kind_subkind == Some LPL.ParserStrong /\
   k.LPL.parser_kind_low > 0 /\
   U32.v pos0 <= U32.v (LPL.slice_of sl).LPL.len /\
   LPL.live_input_buffer h0 sl /\
   live h1 bpos /\
+  live h1 maybe_fail /\
   modifies loc_none h0 h1 /\ (
   if
-    LPL.is_error pos1
+    LPL.is_error err
   then
     stop == true
   else
-    U32.v pos0 <= U64.v pos1 /\
-    U64.v pos1 <= U32.v (LPL.slice_of sl).LPL.len /\
-    R.readable h (LPL.perm_of sl) (LPL.uint64_to_uint32 pos1) (LPL.slice_length sl) /\
+    U32.v pos0 <= U32.v pos1 /\
+    U32.v pos1 <= U32.v (LPL.slice_of sl).LPL.len /\
+    R.readable h (LPL.perm_of sl) (pos1) (LPL.slice_length sl) /\
     (LPL.valid_exact (LPLL.parse_list p) h0 (LPL.slice_of sl) pos0 (LPL.slice_of sl).LPL.len <==>
-     LPL.valid_exact (LPLL.parse_list p) h0 (LPL.slice_of sl) (Cast.uint64_to_uint32 pos1) (LPL.slice_of sl).LPL.len) /\
-    (stop == true ==> U64.v pos1 == U32.v (LPL.slice_of sl).LPL.len)
+     LPL.valid_exact (LPLL.parse_list p) h0 (LPL.slice_of sl) (pos1) (LPL.slice_of sl).LPL.len) /\
+    (stop == true ==> U32.v pos1 == U32.v (LPL.slice_of sl).LPL.len)
   ) /\
-  modifies (l `loc_union` loc_buffer bpos `loc_union` R.loc_perm_from_to (LPL.perm_of sl) pos0 (if LPL.is_error pos1 then LPL.slice_length sl else LPL.uint64_to_uint32 pos1)) h1 h
+  modifies (l `loc_union` B.loc_buffer maybe_fail `loc_union` loc_buffer bpos `loc_union` R.loc_perm_from_to (LPL.perm_of sl) pos0 (if LPL.is_error err then LPL.slice_length sl else pos1)) h1 h
 
 #push-options "--z3rlimit 128"
 
@@ -820,30 +990,32 @@ let validate_list_body
   #inv #l #ar
   (v: validate_with_action_t p inv l ar)
   (g0 g1: Ghost.erased HS.mem)
+  (maybe_fail: pointer U64.t)
   (#len: U32.t)
   (sl: input_buffer_t len)
-  (pos0: LPL.pos_t)
-  (bpos: pointer U64.t)
+  (pos0: U32.t)
+  (bpos: pointer U32.t)
 : HST.Stack bool
-  (requires (fun h -> validate_list_inv p inv l g0 g1 sl (LPL.uint64_to_uint32 pos0) bpos h false))
+  (requires (fun h -> validate_list_inv p inv l g0 g1 maybe_fail sl (pos0) bpos h false))
   (ensures (fun h res h' ->
-    validate_list_inv p inv l g0 g1 sl (LPL.uint64_to_uint32 pos0) bpos h false /\
-    validate_list_inv p inv l g0 g1 sl (LPL.uint64_to_uint32 pos0) bpos h' res
+    validate_list_inv p inv l g0 g1 maybe_fail sl (pos0) bpos h false /\
+    validate_list_inv p inv l g0 g1 maybe_fail sl (pos0) bpos h' res
   ))
 = let h = HST.get () in
   let elementStartPosition = index bpos 0ul in
-  assert (U64.v elementStartPosition <= U32.v (LPL.slice_of sl).LPL.len);
-  if elementStartPosition = Cast.uint32_to_uint64 (LPL.slice_length sl)
+  assert (U32.v elementStartPosition <= U32.v (LPL.slice_of sl).LPL.len);
+  if elementStartPosition = (LPL.slice_length sl)
   then true
   else begin
-    Classical.move_requires (LPLL.valid_exact_list_cons p (Ghost.reveal g0) (LPL.slice_of sl) (LPL.uint64_to_uint32 elementStartPosition)) (LPL.slice_of sl).LPL.len;
-    Classical.move_requires (LPLL.valid_exact_list_cons_recip p (Ghost.reveal g0) (LPL.slice_of sl) (LPL.uint64_to_uint32 elementStartPosition)) (LPL.slice_of sl).LPL.len;
+    Classical.move_requires (LPLL.valid_exact_list_cons p (Ghost.reveal g0) (LPL.slice_of sl) (elementStartPosition)) (LPL.slice_of sl).LPL.len;
+    Classical.move_requires (LPLL.valid_exact_list_cons_recip p (Ghost.reveal g0) (LPL.slice_of sl) (elementStartPosition)) (LPL.slice_of sl).LPL.len;
     let h1 = HST.get () in
     modifies_address_liveness_insensitive_unused_in (Ghost.reveal g0) h1;
-    let elementEndPosition = v sl elementStartPosition in
+    let elementEndPosition = v maybe_fail sl elementStartPosition in
     upd bpos 0ul elementEndPosition;
-    (if LPL.is_success elementEndPosition then R.readable_split h1 (LPL.perm_of sl) (LPL.uint64_to_uint32 elementStartPosition) (LPL.uint64_to_uint32 elementEndPosition) (LPL.slice_length sl));
-    LPL.is_error elementEndPosition
+    let err = B.index maybe_fail 0ul in
+    (if LPL.is_success err then R.readable_split h1 (LPL.perm_of sl) (elementStartPosition) (elementEndPosition) (LPL.slice_length sl));
+    LPL.is_error err
   end
 
 #pop-options
@@ -858,39 +1030,48 @@ let validate_list'
   (#p:parser k t)
   #inv #l #ar
   (v: validate_with_action_t p inv l ar)
+  (maybe_fail: pointer U64.t)
   (#len: U32.t)
   (sl: input_buffer_t len)
-  (pos: U64.t)
-: HST.Stack U64.t
+  (pos: U32.t)
+: HST.Stack U32.t
   (requires (fun h ->
-    U64.v pos <= U32.v (LPL.slice_of sl).LPL.len /\
+    U32.v pos <= U32.v (LPL.slice_of sl).LPL.len /\
     inv (LPL.slice_of sl).LPL.base h /\
     loc_not_unused_in h `loc_includes` l /\
     l `loc_disjoint` LPL.loc_input_buffer sl /\
     address_liveness_insensitive_locs `loc_includes` l /\
-    R.readable h (LPL.perm_of sl) (LPL.uint64_to_uint32 pos) (LPL.slice_of sl).LPL.len /\
+    l `loc_disjoint` B.loc_buffer maybe_fail /\
+    B.loc_buffer maybe_fail `loc_disjoint` LPL.loc_input_buffer sl /\
+    B.live h maybe_fail /\
+    R.readable h (LPL.perm_of sl) (pos) (LPL.slice_of sl).LPL.len /\
     LPL.live_slice h (LPL.slice_of sl)
   ))
   (ensures (fun h res h' ->
+    let err = B.get h' maybe_fail 0 in
     inv (LPL.slice_of sl).LPL.base h' /\
-    (LPL.is_success res ==> (LPL.valid_exact (LPLL.parse_list p) h (LPL.slice_of sl) (LPL.uint64_to_uint32 pos) (LPL.slice_of sl).LPL.len /\ U64.v res == U32.v (LPL.slice_of sl).LPL.len)) /\
-    modifies (l `B.loc_union` R.loc_perm_from_to (LPL.perm_of sl) (LPL.uint64_to_uint32 pos) (if LPL.is_success res then LPL.uint64_to_uint32 res else LPL.slice_length sl)) h h'
+    (LPL.is_success err ==> (LPL.valid_exact (LPLL.parse_list p) h (LPL.slice_of sl) (pos) (LPL.slice_of sl).LPL.len /\ U32.v res == U32.v (LPL.slice_of sl).LPL.len)) /\
+    modifies (l `B.loc_union` B.loc_buffer maybe_fail `B.loc_union` R.loc_perm_from_to (LPL.perm_of sl) (pos) (if LPL.is_success err then res else LPL.slice_length sl)) h h'
   ))
-= let h0 = HST.get () in
-  let g0 = Ghost.hide h0 in
-  HST.push_frame ();
-  let h02 = HST.get () in
-  fresh_frame_modifies h0 h02;
-  let currentPosition = alloca pos 1ul in
-  let h1 = HST.get () in
-  let g1 = Ghost.hide h1 in
-  C.Loops.do_while (validate_list_inv p inv l g0 g1 sl (LPL.uint64_to_uint32 pos) currentPosition) (fun _ -> validate_list_body n v g0 g1 sl pos currentPosition);
-  LPLL.valid_exact_list_nil p h0 (LPL.slice_of sl) (LPL.slice_of sl).LPL.len;
-  let finalPositionOrError = index currentPosition 0ul in
-  HST.pop_frame ();
-  let h' = HST.get () in
-  assert (h' `extends` h0);
-  finalPositionOrError
+= if LPL.is_error (B.index maybe_fail 0ul)
+  then pos
+  else begin
+    let h0 = HST.get () in
+    let g0 = Ghost.hide h0 in
+    HST.push_frame ();
+    let h02 = HST.get () in
+    fresh_frame_modifies h0 h02;
+    let currentPosition = alloca pos 1ul in
+    let h1 = HST.get () in
+    let g1 = Ghost.hide h1 in
+    C.Loops.do_while (validate_list_inv p inv l g0 g1 maybe_fail sl (pos) currentPosition) (fun _ -> validate_list_body n v g0 g1 maybe_fail sl pos currentPosition);
+    LPLL.valid_exact_list_nil p h0 (LPL.slice_of sl) (LPL.slice_of sl).LPL.len;
+    let finalPosition = index currentPosition 0ul in
+    HST.pop_frame ();
+    let h' = HST.get () in
+    assert (h' `extends` h0);
+    finalPosition
+  end
 #pop-options
 
 #push-options "--z3rlimit 32"
@@ -905,19 +1086,174 @@ let validate_nlist
   #inv #l #ar
   (v: validate_with_action_t p inv l ar)
 : Tot (validate_with_action_t (parse_nlist n p) inv l false)
-= fun input pos ->
+= fun maybe_fail input pos ->
   let h = HST.get () in
-  LPL.valid_facts (parse_nlist n p) h (LPL.slice_of input) (LPL.uint64_to_uint32 pos);
-  LPLF.parse_fldata_consumes_all_correct (LPLL.parse_list p) (U32.v n) (LPL.bytes_of_slice_from h (LPL.slice_of input) (LPL.uint64_to_uint32 pos));
-  if (Cast.uint32_to_uint64 (LPL.slice_length input) `U64.sub` pos) `U64.lt` Cast.uint32_to_uint64 n
-  then with_drop_if true inv input (LPL.uint64_to_uint32 pos) (fun _ -> LPL.slice_length input) LPL.validator_error_not_enough_data
-  else begin
-    let listInput = LPL.truncate_input_buffer input (LPL.uint64_to_uint32 pos `U32.add` n) in
-    LPL.valid_exact_equiv (LPLL.parse_list p) h (LPL.slice_of listInput) (LPL.uint64_to_uint32 pos) (LPL.uint64_to_uint32 pos `U32.add` n);
-    R.readable_split h (LPL.perm_of input) (LPL.uint64_to_uint32 pos) (LPL.slice_length listInput) (LPL.slice_length input);
-    with_drop_if true inv input (LPL.uint64_to_uint32 pos) (fun (x: U64.t) -> if LPL.is_success x then LPL.uint64_to_uint32 x else LPL.slice_length input) (validate_list' n v listInput pos)
+  LPL.valid_facts (parse_nlist n p) h (LPL.slice_of input) (pos);
+  LPLF.parse_fldata_consumes_all_correct (LPLL.parse_list p) (U32.v n) (LPL.bytes_of_slice_from h (LPL.slice_of input) (pos));
+  if ((LPL.slice_length input) `U32.sub` pos) `U32.lt` n
+  then begin
+    B.upd maybe_fail 0ul LPL.validator_error_not_enough_data;
+    let h' = HST.get () in
+    assert (h' `extends` h);
+    with_drop_if true inv input (pos) (fun _ -> LPL.slice_length input) pos
+  end else begin
+    let listInput = LPL.truncate_input_buffer input (pos `U32.add` n) in
+    LPL.valid_exact_equiv (LPLL.parse_list p) h (LPL.slice_of listInput) (pos) (pos `U32.add` n);
+    R.readable_split h (LPL.perm_of input) (pos) (LPL.slice_length listInput) (LPL.slice_length input);
+    let res = validate_list' n v maybe_fail listInput pos in
+    let is_success = LPL.is_success (B.index maybe_fail 0ul) in
+    with_drop_if true inv input (pos) (fun x -> if is_success then x else LPL.slice_length input) (res)
   end
 #pop-options
+
+[@unifier_hint_injective]
+inline_for_extraction
+noextract
+let validator_no_read #nz (#k: parser_kind nz) (#t: Type) (p: parser k t) : Tot Type =
+  (maybe_fail: B.pointer U64.t) ->
+  (len: U32.t) ->
+  (sl: Ghost.erased (input_buffer_t len)) ->
+  (pos: U32.t) ->
+  HST.Stack U32.t
+  (requires (fun h ->
+    LPL.live_input_buffer h sl /\
+    U32.v pos <= U32.v len /\
+    B.live h maybe_fail /\
+    B.loc_buffer maybe_fail `B.loc_disjoint` LPL.loc_input_buffer sl
+  ))
+  (ensures (fun h res h' ->
+    B.modifies (B.loc_buffer maybe_fail) h h' /\
+    (LPL.is_success (B.get h' maybe_fail 0) ==> LPL.valid_pos p h (LPL.slice_of sl) (pos) (res)
+  )))
+
+inline_for_extraction
+noextract
+let validate_total_constant_size_no_read
+  #nz
+  (#k: parser_kind nz)
+  (#t: Type)
+  (p: parser k t)
+  (sz: U32.t)
+  (u: unit {
+    let open LP in
+    k.parser_kind_high == Some k.parser_kind_low /\
+    k.parser_kind_low == U32.v sz /\
+    k.parser_kind_metadata == Some ParserKindMetadataTotal
+  })
+: Tot (validator_no_read p)
+= fun maybe_fail len input pos ->
+  let h = HST.get () in
+  [@inline_let] let _ = LPL.valid_total_constant_size h p (U32.v sz) (LPL.slice_of input) (pos) in
+  if U32.lt (len `U32.sub` pos) sz
+  then begin
+    B.upd maybe_fail 0ul LPL.validator_error_not_enough_data;
+    pos
+  end else
+    (pos `U32.add` sz)
+
+inline_for_extraction noextract
+let validate_nlist_total_constant_size_mod_ok (n:U32.t) (#k:parser_kind true) (#t: Type) (p:parser k t)
+  : Pure (validator_no_read (parse_nlist n p))
+  (requires (
+    let open LP in
+    k.parser_kind_subkind == Some ParserStrong /\
+    k.parser_kind_high == Some k.parser_kind_low /\
+    k.parser_kind_metadata == Some ParserKindMetadataTotal /\
+    k.parser_kind_low < 4294967296 /\
+    U32.v n % k.LP.parser_kind_low == 0
+  ))
+  (ensures (fun _ -> True))
+= 
+      (fun maybe_fail len sl pos ->
+         let h = FStar.HyperStack.ST.get () in
+         [@inline_let]
+         let _ =
+           parse_nlist_total_fixed_size_kind_correct n p;
+           LPL.valid_facts (parse_nlist n p) h (LPL.slice_of sl) (pos);
+           LPL.valid_facts (LP.strengthen (LP.total_constant_size_parser_kind (U32.v n)) (parse_nlist n p)) h (LPL.slice_of sl) (pos)
+         in
+         validate_total_constant_size_no_read #false (LP.strengthen (LP.total_constant_size_parser_kind (U32.v n)) (parse_nlist n p)) (n) () maybe_fail len sl pos
+      )
+
+inline_for_extraction noextract
+let validate_nlist_constant_size_mod_ko (n:U32.t) (#k:parser_kind true) #t (p:parser k t)
+  : Pure (validator_no_read (parse_nlist n p))
+  (requires (
+    let open LP in
+    k.parser_kind_subkind == Some ParserStrong /\
+    k.parser_kind_high == Some k.parser_kind_low /\
+    U32.v n % k.LP.parser_kind_low <> 0
+  ))
+  (ensures (fun _ -> True))
+= 
+  (fun maybe_fail len sl pos ->
+     let h = FStar.HyperStack.ST.get () in
+     [@inline_let]
+     let _ =
+       LPL.valid_facts (parse_nlist n p) h (LPL.slice_of sl) (pos)
+     in
+     [@inline_let]
+     let f () : Lemma
+       (requires (LPL.valid (parse_nlist n p) h (LPL.slice_of sl) (pos)))
+       (ensures False)
+     = let sq = LPL.bytes_of_slice_from h (LPL.slice_of sl) (pos) in
+       let sq' = Ghost.hide (Seq.slice sq 0 (U32.v n)) in
+       LowParse.Spec.List.list_length_constant_size_parser_correct p sq' ;
+       let Some (l, _) = LP.parse (parse_nlist n p) sq in
+       assert (U32.v n == FStar.List.Tot.length l `Prims.op_Multiply` k.LP.parser_kind_low) ;
+       FStar.Math.Lemmas.cancel_mul_mod (FStar.List.Tot.length l) k.LP.parser_kind_low ;
+       assert (U32.v n % k.LP.parser_kind_low == 0)
+     in
+     [@inline_let]
+     let _ = Classical.move_requires f () in
+     B.upd maybe_fail 0ul validator_error_list_size_not_multiple;
+     pos
+  )
+
+inline_for_extraction noextract
+let validate_nlist_total_constant_size' (n:U32.t) (#k:parser_kind true) #t (p:parser k t)
+  : Pure (validator_no_read (parse_nlist n p))
+  (requires (
+    let open LP in
+    k.parser_kind_subkind == Some ParserStrong /\
+    k.parser_kind_high == Some k.parser_kind_low /\
+    k.parser_kind_metadata == Some ParserKindMetadataTotal /\
+    k.parser_kind_low < 4294967296
+  ))
+  (ensures (fun _ -> True))
+= fun maybe_fail len sl pos ->
+  if n `U32.rem` U32.uint_to_t k.LP.parser_kind_low = 0ul
+  then validate_nlist_total_constant_size_mod_ok n p maybe_fail len sl pos
+  else validate_nlist_constant_size_mod_ko n p maybe_fail len sl pos
+
+inline_for_extraction noextract
+let validate_nlist_total_constant_size (n_is_const: bool) (n:U32.t) (#k:parser_kind true) (#t: Type) (p:parser k t)
+: Pure (validator_no_read (parse_nlist n p))
+  (requires (
+    let open LP in
+    k.parser_kind_subkind = Some ParserStrong /\
+    k.parser_kind_high = Some k.parser_kind_low /\
+    k.parser_kind_metadata = Some ParserKindMetadataTotal /\
+    k.parser_kind_low < 4294967296
+  ))
+  (ensures (fun _ -> True))
+=
+  if
+    if k.LP.parser_kind_low = 1
+    then true
+    else if n_is_const
+    then U32.v n % k.LP.parser_kind_low = 0
+    else false
+  then
+    validate_nlist_total_constant_size_mod_ok n p
+  else if
+    if n_is_const
+    then U32.v n % k.LP.parser_kind_low <> 0
+    else false
+  then
+    validate_nlist_constant_size_mod_ko n p
+  else
+    validate_nlist_total_constant_size' n p
 
 noextract
 inline_for_extraction
@@ -936,48 +1272,55 @@ let validate_nlist_constant_size_without_actions
     k.parser_kind_metadata = Some ParserKindMetadataTotal &&
     k.parser_kind_low < 4294967296
   then
-    (fun input startPosition ->
+    (fun maybe_fail #len input startPosition ->
       let h = HST.get () in
       assert (forall h' . {:pattern (B.modifies B.loc_none h h')} (B.modifies B.loc_none h h' /\ inv (LPL.slice_of input).LPL.base h) ==> h' `extends` h);
       assert (forall h' . {:pattern (B.modifies B.loc_none h h')} (B.modifies B.loc_none h h' /\ inv (LPL.slice_of input).LPL.base h) ==> inv (LPL.slice_of input).LPL.base h');
-      with_drop_if true inv input (LPL.uint64_to_uint32 startPosition) (fun (y: U64.t) -> if LPL.is_success y then LPL.uint64_to_uint32 y else LPL.slice_length input) (validate_nlist_total_constant_size n_is_const n p (FStar.Ghost.elift1 LPL.slice_of input) (LPL.slice_length input) startPosition)
+      let res = validate_nlist_total_constant_size n_is_const n p maybe_fail (LPL.slice_length input) input startPosition in
+      let is_success = LPL.is_success (B.index maybe_fail 0ul) in
+      let h' = HST.get () in
+      assert (h' `extends` h);
+      with_drop_if true inv input (startPosition) (fun y -> if is_success then y else LPL.slice_length input) (res)
     )
   else
     validate_nlist n v
 
-#push-options "--z3rlimit 16"
+#push-options "--z3rlimit 32"
 
 noextract inline_for_extraction
 let validate_t_at_most' (n:U32.t) (#k:parser_kind true) (#t:_) (#p:parser k t)
                        (#inv:_) (#l:_) (#ar:_) (v:validate_with_action_t p inv l ar)
   : Tot (validate_with_action_t (parse_t_at_most n p) inv l ar)
-  = fun input startPosition ->
+  = fun maybe_fail input startPosition ->
     let h = HST.get () in
     let _ =
-      LPL.valid_weaken kind_t_at_most (LowParse.Spec.FLData.parse_fldata (LPC.nondep_then p LowParse.Spec.Bytes.parse_all_bytes) (U32.v n)) h (LPL.slice_of input) (LPL.uint64_to_uint32 startPosition);
-      LPL.valid_facts (LowParse.Spec.FLData.parse_fldata (LPC.nondep_then p LowParse.Spec.Bytes.parse_all_bytes) (U32.v n)) h (LPL.slice_of input) (LPL.uint64_to_uint32 startPosition)
+      LPL.valid_weaken kind_t_at_most (LowParse.Spec.FLData.parse_fldata (LPC.nondep_then p LowParse.Spec.Bytes.parse_all_bytes) (U32.v n)) h (LPL.slice_of input) (startPosition);
+      LPL.valid_facts (LowParse.Spec.FLData.parse_fldata (LPC.nondep_then p LowParse.Spec.Bytes.parse_all_bytes) (U32.v n)) h (LPL.slice_of input) (startPosition)
     in
-    if (Cast.uint32_to_uint64 (LPL.slice_length input) `U64.sub` startPosition) `U64.lt` Cast.uint32_to_uint64 n
-    then
-      with_drop_if (not ar) inv input (LPL.uint64_to_uint32 startPosition) (fun _ -> LPL.slice_length input)  LPL.validator_error_not_enough_data
-    else
-      [@inline_let] let input' = LPL.truncate_input_buffer input (LPL.uint64_to_uint32 startPosition `U32.add` n) in
-      [@inline_let] let _ = R.readable_split h (LPL.perm_of input) (LPL.uint64_to_uint32 startPosition) (LPL.slice_length input') (LPL.slice_length input) in
+    if ((LPL.slice_length input) `U32.sub` startPosition) `U32.lt` n
+    then begin
+      B.upd maybe_fail 0ul LPL.validator_error_not_enough_data;
+      let h' = HST.get () in
+      assert (h' `extends` h);
+      with_drop_if (not ar) inv input (startPosition) (fun _ -> LPL.slice_length input) startPosition
+    end else
+      [@inline_let] let input' = LPL.truncate_input_buffer input (startPosition `U32.add` n) in
+      [@inline_let] let _ = R.readable_split h (LPL.perm_of input) (startPosition) (LPL.slice_length input') (LPL.slice_length input) in
       [@inline_let] let _ =
-        LPL.valid_facts (LPC.nondep_then p LowParse.Spec.Bytes.parse_all_bytes) h (LPL.slice_of input') (LPL.uint64_to_uint32 startPosition);
-        LPLC.valid_nondep_then h p LowParse.Spec.Bytes.parse_all_bytes (LPL.slice_of input') (LPL.uint64_to_uint32 startPosition)
+        LPL.valid_facts (LPC.nondep_then p LowParse.Spec.Bytes.parse_all_bytes) h (LPL.slice_of input') (startPosition);
+        LPLC.valid_nondep_then h p LowParse.Spec.Bytes.parse_all_bytes (LPL.slice_of input') (startPosition)
       in
       // FIXME: I'd need a name here
-      let positionAfterContents = v input' startPosition in
+      let positionAfterContents = v maybe_fail input' startPosition in
       let h1 = HST.get () in
       let _ = modifies_address_liveness_insensitive_unused_in h h1 in
-      if LPL.is_error positionAfterContents
-      then with_drop_if (not ar) inv input (LPL.uint64_to_uint32 startPosition) (fun _ -> LPL.slice_length input) positionAfterContents
+      if LPL.is_error (B.index maybe_fail 0ul)
+      then with_drop_if (not ar) inv input (startPosition) (fun _ -> LPL.slice_length input) positionAfterContents
       else
         [@inline_let] let _ =
-          LPL.valid_facts LowParse.Spec.Bytes.parse_all_bytes h (LPL.slice_of input') (LPL.uint64_to_uint32 positionAfterContents)
+          LPL.valid_facts LowParse.Spec.Bytes.parse_all_bytes h (LPL.slice_of input') (positionAfterContents)
         in
-        with_drop_if (not ar) inv input (LPL.uint64_to_uint32 startPosition) (fun _ -> LPL.uint64_to_uint32 startPosition `U32.add` n) (startPosition `U64.add` Cast.uint32_to_uint64 n)
+        with_drop_if (not ar) inv input (startPosition) (fun _ -> startPosition `U32.add` n) (startPosition `U32.add` n)
 
 let validate_t_at_most
   n
@@ -988,30 +1331,38 @@ noextract inline_for_extraction
 let validate_t_exact' (n:U32.t) (#nz:bool) (#k:parser_kind nz) (#t:_) (#p:parser k t)
                        (#inv:_) (#l:_) (#ar:_) (v:validate_with_action_t p inv l ar)
   : Tot (validate_with_action_t (parse_t_exact n p) inv l ar)
-  = fun input startPosition ->
+  = fun maybe_fail input startPosition ->
     let h = HST.get () in
     let _ =
-      LPL.valid_weaken kind_t_at_most (LowParse.Spec.FLData.parse_fldata p (U32.v n)) h (LPL.slice_of input) (LPL.uint64_to_uint32 startPosition);
-      LPL.valid_facts (LowParse.Spec.FLData.parse_fldata p (U32.v n)) h (LPL.slice_of input) (LPL.uint64_to_uint32 startPosition)
+      LPL.valid_weaken kind_t_at_most (LowParse.Spec.FLData.parse_fldata p (U32.v n)) h (LPL.slice_of input) (startPosition);
+      LPL.valid_facts (LowParse.Spec.FLData.parse_fldata p (U32.v n)) h (LPL.slice_of input) (startPosition)
     in
-    if (Cast.uint32_to_uint64 (LPL.slice_length input) `U64.sub` startPosition) `U64.lt` Cast.uint32_to_uint64 n
-    then
-    with_drop_if (not ar) inv input (LPL.uint64_to_uint32 startPosition) (fun _ -> LPL.slice_length input) LPL.validator_error_not_enough_data
-    else
-      [@inline_let] let input' = LPL.truncate_input_buffer input (LPL.uint64_to_uint32 startPosition `U32.add` n) in
-      [@inline_let] let _ = R.readable_split h (LPL.perm_of input) (LPL.uint64_to_uint32 startPosition) (LPL.slice_length input') (LPL.slice_length input) in
+    if ((LPL.slice_length input) `U32.sub` startPosition) `U32.lt` n
+    then begin
+      B.upd maybe_fail 0ul LPL.validator_error_not_enough_data;
+      let h1 = HST.get () in
+      assert (h1 `extends` h);
+      with_drop_if (not ar) inv input (startPosition) (fun _ -> LPL.slice_length input) startPosition
+    end else
+      [@inline_let] let input' = LPL.truncate_input_buffer input (startPosition `U32.add` n) in
+      [@inline_let] let _ = R.readable_split h (LPL.perm_of input) (startPosition) (LPL.slice_length input') (LPL.slice_length input) in
       [@inline_let] let _ =
-        LPL.valid_facts p h (LPL.slice_of input') (LPL.uint64_to_uint32 startPosition)
+        LPL.valid_facts p h (LPL.slice_of input') (startPosition)
       in
       // FIXME: I'd need a name here
-      let positionAfterContents = v input' startPosition in
+      let positionAfterContents = v maybe_fail input' startPosition in
       let h1 = HST.get () in
       let _ = modifies_address_liveness_insensitive_unused_in h h1 in
-      if LPL.is_error positionAfterContents
-      then with_drop_if (not ar) inv input (LPL.uint64_to_uint32 startPosition) (fun _ -> LPL.slice_length input) positionAfterContents
-      else if (LPL.uint64_to_uint32 positionAfterContents) <> LPL.slice_length input'
-      then with_drop_if (not ar) inv input (LPL.uint64_to_uint32 startPosition) (fun _ -> LPL.slice_length input) validator_error_unexpected_padding
-      else with_drop_if (not ar) inv input (LPL.uint64_to_uint32 startPosition) (fun _ -> LPL.uint64_to_uint32 startPosition `U32.add` n) (startPosition `U64.add` Cast.uint32_to_uint64 n)
+      if LPL.is_error (B.index maybe_fail 0ul)
+      then with_drop_if (not ar) inv input (startPosition) (fun _ -> LPL.slice_length input) positionAfterContents
+      else if (positionAfterContents) <> LPL.slice_length input'
+      then begin
+        B.upd maybe_fail 0ul validator_error_unexpected_padding;
+        let h2 = HST.get () in
+        assert (h2 `extends` h);
+        with_drop_if (not ar) inv input (startPosition) (fun _ -> LPL.slice_length input) startPosition
+      end
+      else with_drop_if (not ar) inv input (startPosition) (fun _ -> startPosition `U32.add` n) (startPosition `U32.add` n)
 
 #pop-options
 
@@ -1025,9 +1376,9 @@ let validate_with_comment (c:string)
                           #nz (#k:parser_kind nz) #t (#p:parser k t)
                           #inv #l #ar (v:validate_with_action_t p inv l ar)
   : validate_with_action_t p inv l ar
-  = fun input startPosition ->
+  = fun maybe_fail input startPosition ->
     LowParse.Low.Base.comment c;
-    v input startPosition
+    v maybe_fail input startPosition
 
 inline_for_extraction noextract
 let validate_weaken_inv_loc #nz (#k:parser_kind nz) #t (#p:parser k t)
@@ -1063,9 +1414,9 @@ let read_filter #nz
 inline_for_extraction noextract
 let validate____UINT8
   : validator parse____UINT8
-  = fun input startPosition ->
+  = fun maybe_fail input startPosition ->
     LowStar.Comment.comment "Checking that we have enough space for a UINT8, i.e., 1 byte";
-    LowParse.Low.Base.validate_total_constant_size_no_read parse____UINT8 1uL () (Ghost.elift1 LPL.slice_of (Ghost.hide input)) (LPL.slice_length input) startPosition
+    validate_total_constant_size_no_read parse____UINT8 1ul () maybe_fail (LPL.slice_length input) (Ghost.hide input) startPosition
 
 inline_for_extraction noextract
 let read____UINT8
@@ -1075,9 +1426,9 @@ let read____UINT8
 inline_for_extraction noextract
 let validate____UINT16
   : validator parse____UINT16
-  = fun input startPosition ->
+  = fun maybe_fail input startPosition ->
     LowStar.Comment.comment "Checking that we have enough space for a UINT16, i.e., 2 bytes";
-    LowParse.Low.Base.validate_total_constant_size_no_read parse____UINT16 2uL () (Ghost.elift1 LPL.slice_of (Ghost.hide input)) (LPL.slice_length input) startPosition
+    validate_total_constant_size_no_read parse____UINT16 2ul () maybe_fail (LPL.slice_length input) (Ghost.hide input) startPosition
 
 inline_for_extraction noextract
 let read____UINT16
@@ -1088,9 +1439,9 @@ let read____UINT16
 inline_for_extraction noextract
 let validate____UINT32
   : validator parse____UINT32
-  = fun input startPosition ->
+  = fun maybe_fail input startPosition ->
     LowStar.Comment.comment "Checking that we have enough space for a ULONG, i.e., 4 bytes";
-    LowParse.Low.Base.validate_total_constant_size_no_read parse____UINT32 4uL () (Ghost.elift1 LPL.slice_of (Ghost.hide input)) (LPL.slice_length input) startPosition
+    validate_total_constant_size_no_read parse____UINT32 4ul () maybe_fail (LPL.slice_length input) (Ghost.hide input) startPosition
 
 inline_for_extraction noextract
 let read____UINT32
@@ -1100,9 +1451,9 @@ let read____UINT32
 inline_for_extraction noextract
 let validate____UINT64
   : validator parse____UINT64
-  = fun input startPosition ->
+  = fun maybe_fail input startPosition ->
     LowStar.Comment.comment "Checking that we have enough space for a ULONG64, i.e., 8 bytes";
-    LowParse.Low.Base.validate_total_constant_size_no_read parse____UINT64 8uL () (Ghost.elift1 LPL.slice_of (Ghost.hide input)) (LPL.slice_length input) startPosition
+    validate_total_constant_size_no_read parse____UINT64 8ul () maybe_fail (LPL.slice_length input) (Ghost.hide input) startPosition
 
 inline_for_extraction noextract
 let read____UINT64
@@ -1122,15 +1473,18 @@ let read_unit
 inline_for_extraction noextract
 let validate_unit_refinement' (f:unit -> bool) (cf:string)
   : Tot (validate_with_action_t #false (parse_unit `LPC.parse_filter` f) true_inv eloc_none true)
-  = fun input startPosition ->
+  = fun maybe_fail input startPosition ->
       let h = HST.get () in
-      [@inline_let] let _ = LPLC.valid_facts (parse_unit) h (LPL.slice_of input) (LPL.uint64_to_uint32 startPosition) in
-      [@inline_let] let _ = LPLC.valid_filter h parse_unit f (LPL.slice_of input) (LPL.uint64_to_uint32 startPosition) in
+      [@inline_let] let _ = LPLC.valid_facts (parse_unit) h (LPL.slice_of input) (startPosition) in
+      [@inline_let] let _ = LPLC.valid_filter h parse_unit f (LPL.slice_of input) (startPosition) in
       LowStar.Comment.comment cf;
       if f ()
       then
         startPosition
-      else validator_error_constraint_failed
+      else begin
+        B.upd maybe_fail 0ul validator_error_constraint_failed;
+        startPosition
+      end
 
 inline_for_extraction noextract
 let validate_unit_refinement (f:unit -> bool) (cf:string)
@@ -1149,11 +1503,12 @@ let validate_list_up_to_inv
   (p: parser k t)
   (terminator: t)
   (prf: LUT.consumes_if_not_cond (cond_string_up_to terminator) p)
+  (maybe_fail: B.pointer U64.t)
   (#len: U32.t)
   (sl: input_buffer_t len)
   (pos0: U32.t)
   (h0: HS.mem)
-  (bpos: B.pointer U64.t)
+  (bpos: B.pointer U32.t)
   (h: HS.mem)
   (stop: bool)
 : GTot Type0
@@ -1164,12 +1519,13 @@ let validate_list_up_to_inv
   live_input_buffer h0 sl /\
   live_input_buffer h sl /\
   B.loc_disjoint (LPL.loc_input_buffer sl) (B.loc_buffer bpos) /\
-  U32.v pos0 <= U64.v pos /\
-  begin if is_success pos
+  B.live h0 maybe_fail /\
+  B.loc_disjoint (LPL.loc_input_buffer sl `B.loc_union` B.loc_buffer bpos) (B.loc_buffer maybe_fail) /\
+  begin if is_success (B.get h maybe_fail 0)
   then
-    let pos = uint64_to_uint32 pos in
+    U32.v pos0 <= U32.v pos /\
     U32.v pos <= U32.v (slice_of sl).len /\
-    B.modifies (B.loc_buffer bpos `B.loc_union` R.loc_perm_from_to (perm_of sl) pos0 pos) h0 h /\
+    B.modifies (B.loc_buffer maybe_fail `B.loc_union` B.loc_buffer bpos `B.loc_union` R.loc_perm_from_to (perm_of sl) pos0 pos) h0 h /\
     R.unreadable h (perm_of sl) pos0 pos /\
     R.readable h (perm_of sl) pos (slice_of sl).len /\
     begin if stop
@@ -1183,13 +1539,13 @@ let validate_list_up_to_inv
     end
   else
     U32.v pos0 <= U32.v (slice_of sl).len /\
-    B.modifies (B.loc_buffer bpos `B.loc_union` R.loc_perm_from_to (perm_of sl) pos0 (slice_of sl).len) h0 h /\
+    B.modifies (B.loc_buffer maybe_fail `B.loc_union` B.loc_buffer bpos `B.loc_union` R.loc_perm_from_to (perm_of sl) pos0 (slice_of sl).len) h0 h /\
     R.unreadable h (perm_of sl) pos0 (slice_of sl).len /\
     stop == true /\
     True // (~ (valid q h0 (slice_of sl) pos0)) // we lost completeness because of actions
   end
 
-#push-options "--z3rlimit 16"
+#push-options "--z3rlimit 32"
 
 inline_for_extraction
 let validate_list_up_to_body
@@ -1200,42 +1556,43 @@ let validate_list_up_to_body
   (prf: LUT.consumes_if_not_cond (cond_string_up_to terminator) p)
   (v: validator p)
   (r: leaf_reader p)
+  (maybe_fail: B.pointer U64.t)
   (#len: U32.t)
   (sl: input_buffer_t len)
   (pos0: U32.t)
   (h0: HS.mem)
-  (bpos: B.pointer U64.t)
+  (bpos: B.pointer U32.t)
 : HST.Stack bool
   (requires (fun h ->
-    validate_list_up_to_inv p terminator prf sl pos0 h0 bpos h false
+    validate_list_up_to_inv p terminator prf maybe_fail sl pos0 h0 bpos h false
   ))
   (ensures (fun h stop h' ->
-    validate_list_up_to_inv p terminator prf sl pos0 h0 bpos h false /\
-    validate_list_up_to_inv p terminator prf sl pos0 h0 bpos h' stop
+    validate_list_up_to_inv p terminator prf maybe_fail sl pos0 h0 bpos h false /\
+    validate_list_up_to_inv p terminator prf maybe_fail sl pos0 h0 bpos h' stop
   ))
 =
   let open LPL in
   let open LUT in
   let h = HST.get () in
   let pos = B.index bpos 0ul in
-  valid_facts (parse_list_up_to (cond_string_up_to terminator) p prf) h0 (slice_of sl) (uint64_to_uint32 pos);
-  parse_list_up_to_eq (cond_string_up_to terminator) p prf (bytes_of_slice_from h0 (slice_of sl) (uint64_to_uint32 pos));
-  valid_facts p h0 (slice_of sl) (uint64_to_uint32 pos);
-  let pos1 = v sl pos in
+  valid_facts (parse_list_up_to (cond_string_up_to terminator) p prf) h0 (slice_of sl) (pos);
+  parse_list_up_to_eq (cond_string_up_to terminator) p prf (bytes_of_slice_from h0 (slice_of sl) (pos));
+  valid_facts p h0 (slice_of sl) (pos);
+  let pos1 = v maybe_fail sl pos in
   B.upd bpos 0ul pos1;
-  if is_error pos1
+  if is_error (B.index maybe_fail 0ul)
   then begin
-    drop sl (uint64_to_uint32 pos) (slice_length sl);
+    drop sl (pos) (slice_length sl);
     let h = HST.get () in
-    R.unreadable_split h (perm_of sl) pos0 (uint64_to_uint32 pos) (slice_length sl);
+    R.unreadable_split h (perm_of sl) pos0 (pos) (slice_length sl);
     true
   end else begin
-    valid_facts (parse_list_up_to (cond_string_up_to terminator) p prf) h0 (slice_of sl) (uint64_to_uint32 pos1);
+    valid_facts (parse_list_up_to (cond_string_up_to terminator) p prf) h0 (slice_of sl) (pos1);
     let h = HST.get () in
-    R.readable_split h (perm_of sl) (uint64_to_uint32 pos) (uint64_to_uint32 pos1) (slice_length sl);
-    let x = r sl (uint64_to_uint32 pos) in
+    R.readable_split h (perm_of sl) (pos) (pos1) (slice_length sl);
+    let x = r sl (pos) in
     let h = HST.get () in
-    R.unreadable_split h (perm_of sl) pos0 (uint64_to_uint32 pos) (uint64_to_uint32 pos1);
+    R.unreadable_split h (perm_of sl) pos0 (pos) (pos1);
     cond_string_up_to terminator x
   end
 
@@ -1251,18 +1608,24 @@ let validate_list_up_to
   (prf: LUT.consumes_if_not_cond (cond_string_up_to terminator) p)
 : Tot (validate_with_action_t #true (LUT.parse_list_up_to (cond_string_up_to terminator) p prf) true_inv eloc_none false)
 =
-  fun sl pos ->
-  HST.push_frame ();
-  let bpos = B.alloca pos 1ul in
-  let h2 = HST.get () in
-  R.unreadable_empty h2 (LPL.perm_of sl) (LPL.uint64_to_uint32 pos);
-  C.Loops.do_while
-    (validate_list_up_to_inv p terminator prf sl (LPL.uint64_to_uint32 pos) h2 bpos)
-    (fun _ -> validate_list_up_to_body terminator prf v r sl (LPL.uint64_to_uint32 pos) h2 bpos)
-    ;
-  let res = B.index bpos 0ul in
-  HST.pop_frame ();
-  res
+  fun maybe_fail sl pos ->
+  if LPL.is_error (B.index maybe_fail 0ul)
+  then begin
+    LPL.drop sl (pos) (LPL.slice_length sl);
+    pos
+  end else begin
+    HST.push_frame ();
+    let bpos = B.alloca pos 1ul in
+    let h2 = HST.get () in
+    R.unreadable_empty h2 (LPL.perm_of sl) (pos);
+    C.Loops.do_while
+      (validate_list_up_to_inv p terminator prf maybe_fail sl (pos) h2 bpos)
+      (fun _ -> validate_list_up_to_body terminator prf v r maybe_fail sl (pos) h2 bpos)
+      ;
+    let res = B.index bpos 0ul in
+    HST.pop_frame ();
+    res
+  end
 
 #pop-options
 
@@ -1280,7 +1643,7 @@ let action_return
       #nz (#k:parser_kind nz) (#t:Type) (#p:parser k t)
       (#a:Type) (x:a)
   : action p true_inv eloc_none false a
-  = fun input startPosition endPosition -> x
+  = fun _ input startPosition endPosition -> x
 
 noextract
 inline_for_extraction
@@ -1292,13 +1655,13 @@ let action_bind
       (#invg:slice_inv) (#lg:eloc) #bg
       (#b:Type) (g: (a -> action p invg lg bg b))
   : Tot (action p (conj_inv invf invg) (eloc_union lf lg) (bf || bg) b)
-  = fun input startPosition endPosition ->
+  = fun maybe_fail input startPosition endPosition ->
     let h0 = HST.get () in
     [@(rename_let ("" ^ name))]
-    let x = f input startPosition endPosition in
+    let x = f maybe_fail input startPosition endPosition in
     let h1 = HST.get () in
     modifies_address_liveness_insensitive_unused_in h0 h1;
-    g x input startPosition endPosition
+    g x maybe_fail input startPosition endPosition
 
 noextract
 inline_for_extraction
@@ -1309,12 +1672,12 @@ let action_seq
       (#invg:slice_inv) (#lg:eloc) #bg
       (#b:Type) (g: action p invg lg bg b)
   : Tot (action p (conj_inv invf invg) (eloc_union lf lg) (bf || bg) b)
-  = fun input startPosition endPosition ->
+  = fun maybe_fail input startPosition endPosition ->
     let h0 = HST.get () in
-    let _ = f input startPosition endPosition in
+    let _ = f maybe_fail input startPosition endPosition in
     let h1 = HST.get () in
     modifies_address_liveness_insensitive_unused_in h0 h1;
-    g input startPosition endPosition
+    g maybe_fail input startPosition endPosition
 
 noextract
 inline_for_extraction
@@ -1326,24 +1689,24 @@ let action_ite
       (#invg:slice_inv) (#lg:eloc) #bg
       (else_: squash (not guard) -> action p invg lg bg a)
   : action p (conj_inv invf invg) (eloc_union lf lg) (bf || bg) a
-  = fun input startPosition endPosition ->
+  = fun maybe_fail input startPosition endPosition ->
       if guard 
-      then then_ () input startPosition endPosition 
-      else else_ () input startPosition endPosition
+      then then_ () maybe_fail input startPosition endPosition 
+      else else_ () maybe_fail input startPosition endPosition
 
 noextract
 inline_for_extraction
 let action_abort
       #nz (#k:parser_kind nz) (#t:Type) (#p:parser k t)
   : action p true_inv eloc_none false bool
-  = fun input startPosition endPosition -> false
+  = fun _ input startPosition endPosition -> false
 
 noextract
 inline_for_extraction
 let action_field_pos
       #nz (#k:parser_kind nz) (#t:Type) (#p:parser k t) (u:unit)
    : action p true_inv eloc_none false U32.t
-   = fun _ startPosition _ -> LPL.uint64_to_uint32 startPosition
+   = fun _ _ startPosition _ -> startPosition
 
 
 noextract
@@ -1351,9 +1714,9 @@ inline_for_extraction
 let action_field_ptr
       #nz (#k:parser_kind nz) (#t:Type) (#p:parser k t) (u:unit)
    : action p true_inv eloc_none true LPL.puint8
-   = fun input startPosition _ ->
+   = fun _ input startPosition _ ->
        let open LowParse.Slice in
-       LPL.offset input (LPL.uint64_to_uint32 startPosition)
+       LPL.offset input (startPosition)
 
 noextract
 inline_for_extraction
@@ -1361,7 +1724,7 @@ let action_deref
       #nz (#k:parser_kind nz) (#t:Type) (#p:parser k t)
       (#a:_) (x:B.pointer a)
    : action p (ptr_inv x) loc_none false a
-   = fun _ _ _ -> !*x
+   = fun _ _ _ _ -> !*x
 
 noextract
 inline_for_extraction
@@ -1369,7 +1732,7 @@ let action_assignment
       #nz (#k:parser_kind nz) (#t:Type) (#p:parser k t)
       (#a:_) (x:B.pointer a) (v:a)
    : action p (ptr_inv x) (ptr_loc x) false unit
-   = fun _ _ _ -> x *= v
+   = fun _ _ _ _ -> x *= v
 
 (* FIXME: This is now unsound.
 noextract
