src/3d/prelude/ResultOps.fst
@@ -2,6 +2,8 @@ module ResultOps
 module U32 = FStar.UInt32
 module U64 = FStar.UInt64
 module LPL = LowParse.Low.Base
+module HST = FStar.HyperStack.ST
+module B = LowStar.Buffer
 module BF = LowParse.BitFields
 let result = U64.t
 let field_id = x:U64.t{ 0 < U64.v x /\ U64.v x < pow2 16}
@@ -38,19 +40,6 @@ let validator_error_constraint_failed : LPL.validator_error = normalize_term (LP
 [@ CMacro ]
 let validator_error_unexpected_padding : LPL.validator_error = normalize_term (LPL.set_validator_error_kind 0uL 7uL)
 
-[@ CInline ]
-let check_constraint_ok (ok:bool) (position:U64.t) : Tot U64.t =
-      if ok
-      then position
-      else validator_error_constraint_failed
-
-[@ CInline ]
-let check_constraint_ok_with_field_id (ok:bool) (startPosition: LPL.pos_t) (endPosition:U64.t) (fieldId: field_id) : Tot U64.t =
-      if ok
-      then endPosition
-      else LPL.set_validator_error_pos_and_code validator_error_constraint_failed startPosition fieldId
-
-////////////////////////////////////////////////////////////////////////////////
 // Some generic helpers
 ////////////////////////////////////////////////////////////////////////////////
 [@ CInline ]
@@ -59,3 +48,8 @@ let is_range_okay (size offset access_size:U32.t)
   = let open U32 in
     size >=^ access_size &&
     size -^ access_size >=^ offset
+
+
+module B = LowStar.Buffer
+module HST = FStar.HyperStack.ST
+module LPL = LowParse.Low.Base
